SeparationLogic/examples/QCP_demos_LLM/kosaraju_rel_goal.v
@@ -116,6 +116,7 @@ forall (timer_p_pre: Z) (fin_pre: Z) (vis1_pre: Z) (radj_pre: Z) (n_pre: Z) (u_p
   **  ((( &( "vis1" ) )) # Ptr  |-> vis1_pre)
   **  ((( &( "fin" ) )) # Ptr  |-> fin_pre)
   **  ((( &( "timer_p" ) )) # Ptr  |-> timer_p_pre)
+  **  (((radj_pre + (u_pre * sizeof(PTR) ) )) # Ptr  |-> head)
   **  (SllPtrArray.missing_i radj_pre n_pre u_pre head radj_rows_low_level_spec )
   **  ((( &( "cur" ) )) # Ptr  |-> cur)
   **  (sllseg head cur processed )
@@ -136,6 +137,7 @@ forall (radj_rows_low_level_spec: (@list (@list Z))) (X_low_level_spec: (unit ->
   **  ((( &( "n" ) )) # Int  |-> n)
   **  ((( &( "u" ) )) # Int  |-> u)
   **  ((( &( "radj" ) )) # Ptr  |-> radj)
+  **  (((radj + (u * sizeof(PTR) ) )) # Ptr  |-> head)
   **  (SllPtrArray.missing_i radj n u head radj_rows_low_level_spec )
   **  (sllseg head cur processed )
   **  ((&((cur)  # "list" ->ₛ "data")) # Int  |-> vdata)
@@ -160,6 +162,7 @@ forall (timer_p_pre: Z) (fin_pre: Z) (vis1_pre: Z) (radj_pre: Z) (n_pre: Z) (u_p
   **  ((( &( "vis1" ) )) # Ptr  |-> vis1_pre)
   **  ((( &( "fin" ) )) # Ptr  |-> fin_pre)
   **  ((( &( "timer_p" ) )) # Ptr  |-> timer_p_pre)
+  **  (((radj_pre + (u_pre * sizeof(PTR) ) )) # Ptr  |-> head)
   **  (SllPtrArray.missing_i radj_pre n_pre u_pre head radj_rows_low_level_spec )
   **  ((( &( "cur" ) )) # Ptr  |-> cur)
   **  (sllseg head cur processed )
@@ -182,6 +185,7 @@ forall (timer_p_pre: Z) (fin_pre: Z) (vis1_pre: Z) (radj_pre: Z) (n_pre: Z) (u_p
   **  ((( &( "fin" ) )) # Ptr  |-> fin_pre)
   **  ((( &( "timer_p" ) )) # Ptr  |-> timer_p_pre)
   **  ((( &( "t0" ) )) # Int  |-> timer_m)
+  **  (((radj_pre + (u_pre * sizeof(PTR) ) )) # Ptr  |-> head)
   **  (SllPtrArray.missing_i radj_pre n_pre u_pre head radj_rows_low_level_spec )
   **  (sll head (Znth (u_pre) (radj_rows_low_level_spec) ((@nil Z))) )
   **  ((( &( "cur" ) )) # Ptr  |-> 0)
@@ -203,6 +207,7 @@ forall (timer_p_pre: Z) (fin_pre: Z) (vis1_pre: Z) (radj_pre: Z) (n_pre: Z) (u_p
   **  ((( &( "fin" ) )) # Ptr  |-> fin_pre)
   **  ((( &( "timer_p" ) )) # Ptr  |-> timer_p_pre)
   **  ((( &( "t0" ) )) # Int  |-> timer_m)
+  **  (((radj_pre + (u_pre * sizeof(PTR) ) )) # Ptr  |-> head)
   **  (SllPtrArray.missing_i radj_pre n_pre u_pre head radj_rows_low_level_spec )
   **  (sll head (Znth (u_pre) (radj_rows_low_level_spec) ((@nil Z))) )
   **  ((( &( "cur" ) )) # Ptr  |-> 0)
@@ -222,6 +227,7 @@ forall (timer_p_pre: Z) (fin_pre: Z) (vis1_pre: Z) (radj_pre: Z) (n_pre: Z) (u_p
   **  ((( &( "fin" ) )) # Ptr  |-> fin_pre)
   **  ((( &( "timer_p" ) )) # Ptr  |-> timer_p_pre)
   **  ((( &( "t0" ) )) # Int  |-> timer_m)
+  **  (((radj_pre + (u_pre * sizeof(PTR) ) )) # Ptr  |-> head)
   **  (SllPtrArray.missing_i radj_pre n_pre u_pre head radj_rows_low_level_spec )
   **  (sll head (Znth (u_pre) (radj_rows_low_level_spec) ((@nil Z))) )
   **  ((( &( "cur" ) )) # Ptr  |-> 0)
@@ -242,6 +248,7 @@ forall (timer_p_pre: Z) (fin_pre: Z) (vis1_pre: Z) (radj_pre: Z) (n_pre: Z) (u_p
   **  ((( &( "fin" ) )) # Ptr  |-> fin_pre)
   **  ((( &( "timer_p" ) )) # Ptr  |-> timer_p_pre)
   **  ((( &( "t0" ) )) # Int  |-> timer_m)
+  **  (((radj_pre + (u_pre * sizeof(PTR) ) )) # Ptr  |-> head)
   **  (SllPtrArray.missing_i radj_pre n_pre u_pre head radj_rows_low_level_spec )
   **  (sll head (Znth (u_pre) (radj_rows_low_level_spec) ((@nil Z))) )
   **  ((( &( "cur" ) )) # Ptr  |-> 0)
@@ -261,6 +268,7 @@ forall (timer_p_pre: Z) (fin_pre: Z) (vis1_pre: Z) (radj_pre: Z) (n_pre: Z) (u_p
   **  ((( &( "fin" ) )) # Ptr  |-> fin_pre)
   **  ((( &( "timer_p" ) )) # Ptr  |-> timer_p_pre)
   **  ((( &( "t0" ) )) # Int  |-> timer_m)
+  **  (((radj_pre + (u_pre * sizeof(PTR) ) )) # Ptr  |-> head)
   **  (SllPtrArray.missing_i radj_pre n_pre u_pre head radj_rows_low_level_spec )
   **  (sll head (Znth (u_pre) (radj_rows_low_level_spec) ((@nil Z))) )
   **  ((( &( "cur" ) )) # Ptr  |-> 0)
@@ -280,6 +288,7 @@ forall (timer_p_pre: Z) (fin_pre: Z) (vis1_pre: Z) (radj_pre: Z) (n_pre: Z) (u_p
   **  ((( &( "fin" ) )) # Ptr  |-> fin_pre)
   **  ((( &( "timer_p" ) )) # Ptr  |-> timer_p_pre)
   **  ((( &( "t0" ) )) # Int  |-> timer_m)
+  **  (((radj_pre + (u_pre * sizeof(PTR) ) )) # Ptr  |-> head)
   **  (SllPtrArray.missing_i radj_pre n_pre u_pre head radj_rows_low_level_spec )
   **  (sll head (Znth (u_pre) (radj_rows_low_level_spec) ((@nil Z))) )
   **  ((( &( "cur" ) )) # Ptr  |-> 0)
@@ -303,7 +312,8 @@ forall (timer_p_pre: Z) (fin_pre: Z) (vis1_pre: Z) (radj_pre: Z) (n_pre: Z) (u_p
   &&  “ (0 <= u_pre) ” 
   &&  “ (u_pre < n_pre) ” 
   &&  “ (n_pre <= INT_MAX) ”
-  &&  (SllPtrArray.missing_i radj_pre n_pre u_pre head radj_rows_low_level_spec )
+  &&  (((radj_pre + (u_pre * sizeof(PTR) ) )) # Ptr  |-> head)
+  **  (SllPtrArray.missing_i radj_pre n_pre u_pre head radj_rows_low_level_spec )
   **  (sllseg head row_ptr processed )
   **  (sll row_ptr rem )
   **  (IntArray.full vis1_pre n_pre vis1_m )
@@ -311,17 +321,16 @@ forall (timer_p_pre: Z) (fin_pre: Z) (vis1_pre: Z) (radj_pre: Z) (n_pre: Z) (u_p
   **  (IntArray.full timer_p_pre 1 (cons (timer_m) ((@nil Z))) )
 ) \/
 (
-forall (radj_pre: Z) (n_pre: Z) (u_pre: Z) (radj_rows_low_level_spec: (@list (@list Z))) (X_low_level_spec: (unit -> (KSt -> Prop))) (timer_v_low_level_spec: Z) (fin_l_low_level_spec: (@list Z)) (vis1_l_low_level_spec: (@list Z)) (g_low_level_spec: AdjGraph) (row_ptr: Z) (PreH1 : (safeExec (pre_dfs1 (g_low_level_spec) (vis1_l_low_level_spec) (fin_l_low_level_spec) (timer_v_low_level_spec)) (dfs_finish (u_pre)) X_low_level_spec )) (PreH2 : (0 <= u_pre)) (PreH3 : (u_pre < n_pre)) (PreH4 : (n_pre <= INT_MAX)) ,
-  (SllPtrArray.full radj_pre n_pre radj_rows_low_level_spec )
+forall (n_pre: Z) (u_pre: Z) (radj_rows_low_level_spec: (@list (@list Z))) (X_low_level_spec: (unit -> (KSt -> Prop))) (timer_v_low_level_spec: Z) (fin_l_low_level_spec: (@list Z)) (vis1_l_low_level_spec: (@list Z)) (g_low_level_spec: AdjGraph) (row_ptr: Z) (row_ptr_2: Z)  __default__List_Z (PreH1 : (safeExec (pre_dfs1 (g_low_level_spec) (vis1_l_low_level_spec) (fin_l_low_level_spec) (timer_v_low_level_spec)) (dfs_finish (u_pre)) X_low_level_spec )) (PreH2 : (0 <= u_pre)) (PreH3 : (u_pre < n_pre)) (PreH4 : (n_pre <= INT_MAX)) ,
+  (sll row_ptr_2 (Znth u_pre radj_rows_low_level_spec __default__List_Z) )
 |--
-  EX (rem: (@list Z))  (head: Z)  (timer_m: Z)  (processed: (@list Z)) ,
+  EX (rem: (@list Z))  (timer_m: Z)  (processed: (@list Z)) ,
   “ ((cons (timer_v_low_level_spec) ((@nil Z))) = (cons (timer_m) ((@nil Z)))) ” 
   &&  “ (safeExec (pre_dfs1 (g_low_level_spec) ((replace_Znth (u_pre) (1) (vis1_l_low_level_spec))) (fin_l_low_level_spec) (timer_m)) (dfs_finish_from (u_pre) ((edges_of (u_pre) (processed)))) X_low_level_spec ) ” 
   &&  “ (0 <= u_pre) ” 
   &&  “ (u_pre < n_pre) ” 
   &&  “ (n_pre <= INT_MAX) ”
-  &&  (SllPtrArray.missing_i radj_pre n_pre u_pre head radj_rows_low_level_spec )
-  **  (sllseg head row_ptr processed )
+  &&  (sllseg row_ptr_2 row_ptr processed )
   **  (sll row_ptr rem )
 ).
 
@@ -329,6 +338,7 @@ Definition dfs1_entail_wit_2 :=
 (
 forall (timer_p_pre: Z) (fin_pre: Z) (vis1_pre: Z) (radj_pre: Z) (n_pre: Z) (u_pre: Z) (radj_rows_low_level_spec: (@list (@list Z))) (X_low_level_spec: (unit -> (KSt -> Prop))) (g_low_level_spec: AdjGraph) (cur: Z) (head: Z) (processed: (@list Z)) (rem: (@list Z)) (vis1_m: (@list Z)) (fin_m: (@list Z)) (timer_m: Z) (PreH1 : (cur <> 0)) (PreH2 : (safeExec (pre_dfs1 (g_low_level_spec) (vis1_m) (fin_m) (timer_m)) (dfs_finish_from (u_pre) ((edges_of (u_pre) (processed)))) X_low_level_spec )) (PreH3 : (0 <= u_pre)) (PreH4 : (u_pre < n_pre)) (PreH5 : (n_pre <= INT_MAX)) ,
   ((( &( "v" ) )) # Int  |->_)
+  **  (((radj_pre + (u_pre * sizeof(PTR) ) )) # Ptr  |-> head)
   **  (SllPtrArray.missing_i radj_pre n_pre u_pre head radj_rows_low_level_spec )
   **  (sllseg head cur processed )
   **  (sll cur rem )
@@ -344,6 +354,7 @@ forall (timer_p_pre: Z) (fin_pre: Z) (vis1_pre: Z) (radj_pre: Z) (n_pre: Z) (u_p
   &&  “ (rem = (cons (vdata) (rest))) ” 
   &&  “ (safeExec (pre_dfs1 (g_low_level_spec) (vis1_m) (fin_m) (timer_m)) (dfs_finish_from (u_pre) ((edges_of (u_pre) (processed)))) X_low_level_spec ) ”
   &&  ((( &( "v" ) )) # Int  |-> vdata)
+  **  (((radj_pre + (u_pre * sizeof(PTR) ) )) # Ptr  |-> head)
   **  (SllPtrArray.missing_i radj_pre n_pre u_pre head radj_rows_low_level_spec )
   **  (sllseg head cur processed )
   **  ((&((cur)  # "list" ->ₛ "data")) # Int  |-> vdata)
@@ -396,6 +407,7 @@ forall (timer_p_pre: Z) (fin_pre: Z) (vis1_pre: Z) (radj_pre: Z) (n_pre: Z) (u_p
   **  ((( &( "n" ) )) # Int  |-> n)
   **  ((( &( "u" ) )) # Int  |-> u)
   **  ((( &( "radj" ) )) # Ptr  |-> radj)
+  **  (((radj + (u * sizeof(PTR) ) )) # Ptr  |-> head)
   **  (SllPtrArray.missing_i radj n u head radj_rows_low_level_spec )
   **  (sllseg head cur processed )
   **  ((&((cur)  # "list" ->ₛ "data")) # Int  |-> vdata)
@@ -429,6 +441,7 @@ forall (timer_p_pre: Z) (fin_pre: Z) (vis1_pre: Z) (radj_pre: Z) (n_pre: Z) (u_p
 (
 forall (timer_p_pre: Z) (fin_pre: Z) (vis1_pre: Z) (radj_pre: Z) (n_pre: Z) (u_pre: Z) (radj_rows_low_level_spec: (@list (@list Z))) (X_low_level_spec: (unit -> (KSt -> Prop))) (g_low_level_spec: AdjGraph) (head: Z) (processed: (@list Z)) (rem: (@list Z)) (vis1_m: (@list Z)) (fin_m: (@list Z)) (timer_m: Z) (vdata: Z) (rest: (@list Z)) (next_ptr: Z) (cur: Z) (n: Z) (u: Z) (radj: Z) (vis1: Z) (fin: Z) (timer_p: Z) (PreH1 : (vdata <= INT_MAX)) (PreH2 : (vdata >= INT_MIN)) (PreH3 : ((Znth vdata vis1_m 0) = 0)) (PreH4 : (cur <> 0)) (PreH5 : (0 <= vdata)) (PreH6 : (vdata < n)) (PreH7 : (n <= INT_MAX)) (PreH8 : (rem = (cons (vdata) (rest)))) (PreH9 : (safeExec (pre_dfs1 (g_low_level_spec) (vis1_m) (fin_m) (timer_m)) (dfs_finish_from (u) ((edges_of (u) (processed)))) X_low_level_spec )) ,
   (IntArray.full vis1 n vis1_m )
+  **  (((radj + (u * sizeof(PTR) ) )) # Ptr  |-> head)
   **  (SllPtrArray.missing_i radj n u head radj_rows_low_level_spec )
   **  (sllseg head cur processed )
   **  ((&((cur)  # "list" ->ₛ "data")) # Int  |-> vdata)
@@ -458,6 +471,7 @@ forall (timer_p_pre: Z) (fin_pre: Z) (vis1_pre: Z) (radj_pre: Z) (n_pre: Z) (u_p
 Definition dfs1_entail_wit_3_split_goal_1 := 
 forall (radj_rows_low_level_spec: (@list (@list Z))) (X_low_level_spec: (unit -> (KSt -> Prop))) (g_low_level_spec: AdjGraph) (head: Z) (processed: (@list Z)) (rem: (@list Z)) (vis1_m: (@list Z)) (fin_m: (@list Z)) (timer_m: Z) (vdata: Z) (rest: (@list Z)) (next_ptr: Z) (cur: Z) (n: Z) (u: Z) (radj: Z) (vis1: Z) (fin: Z) (timer_p: Z) (PreH1 : (vdata <= INT_MAX)) (PreH2 : (vdata >= INT_MIN)) (PreH3 : ((Znth vdata vis1_m 0) = 0)) (PreH4 : (cur <> 0)) (PreH5 : (0 <= vdata)) (PreH6 : (vdata < n)) (PreH7 : (n <= INT_MAX)) (PreH8 : (rem = (cons (vdata) (rest)))) (PreH9 : (safeExec (pre_dfs1 (g_low_level_spec) (vis1_m) (fin_m) (timer_m)) (dfs_finish_from (u) ((edges_of (u) (processed)))) X_low_level_spec )) ,
   (IntArray.full vis1 n vis1_m )
+  **  (((radj + (u * sizeof(PTR) ) )) # Ptr  |-> head)
   **  (SllPtrArray.missing_i radj n u head radj_rows_low_level_spec )
   **  (sllseg head cur processed )
   **  ((&((cur)  # "list" ->ₛ "data")) # Int  |-> vdata)
@@ -472,6 +486,7 @@ forall (radj_rows_low_level_spec: (@list (@list Z))) (X_low_level_spec: (unit ->
 Definition dfs1_entail_wit_3_split_goal_2 := 
 forall (radj_rows_low_level_spec: (@list (@list Z))) (X_low_level_spec: (unit -> (KSt -> Prop))) (g_low_level_spec: AdjGraph) (head: Z) (processed: (@list Z)) (rem: (@list Z)) (vis1_m: (@list Z)) (fin_m: (@list Z)) (timer_m: Z) (vdata: Z) (rest: (@list Z)) (next_ptr: Z) (cur: Z) (n: Z) (u: Z) (radj: Z) (vis1: Z) (fin: Z) (timer_p: Z) (PreH1 : (vdata <= INT_MAX)) (PreH2 : (vdata >= INT_MIN)) (PreH3 : ((Znth vdata vis1_m 0) = 0)) (PreH4 : (cur <> 0)) (PreH5 : (0 <= vdata)) (PreH6 : (vdata < n)) (PreH7 : (n <= INT_MAX)) (PreH8 : (rem = (cons (vdata) (rest)))) (PreH9 : (safeExec (pre_dfs1 (g_low_level_spec) (vis1_m) (fin_m) (timer_m)) (dfs_finish_from (u) ((edges_of (u) (processed)))) X_low_level_spec )) ,
   (IntArray.full vis1 n vis1_m )
+  **  (((radj + (u * sizeof(PTR) ) )) # Ptr  |-> head)
   **  (SllPtrArray.missing_i radj n u head radj_rows_low_level_spec )
   **  (sllseg head cur processed )
   **  ((&((cur)  # "list" ->ₛ "data")) # Int  |-> vdata)
@@ -486,6 +501,7 @@ forall (radj_rows_low_level_spec: (@list (@list Z))) (X_low_level_spec: (unit ->
 Definition dfs1_entail_wit_3_split_goal_3 := 
 forall (n_pre: Z) (radj_rows_low_level_spec: (@list (@list Z))) (X_low_level_spec: (unit -> (KSt -> Prop))) (g_low_level_spec: AdjGraph) (head: Z) (processed: (@list Z)) (rem: (@list Z)) (vis1_m: (@list Z)) (fin_m: (@list Z)) (timer_m: Z) (vdata: Z) (rest: (@list Z)) (next_ptr: Z) (cur: Z) (n: Z) (u: Z) (radj: Z) (vis1: Z) (fin: Z) (timer_p: Z) (PreH1 : (vdata <= INT_MAX)) (PreH2 : (vdata >= INT_MIN)) (PreH3 : ((Znth vdata vis1_m 0) = 0)) (PreH4 : (cur <> 0)) (PreH5 : (0 <= vdata)) (PreH6 : (vdata < n)) (PreH7 : (n <= INT_MAX)) (PreH8 : (rem = (cons (vdata) (rest)))) (PreH9 : (safeExec (pre_dfs1 (g_low_level_spec) (vis1_m) (fin_m) (timer_m)) (dfs_finish_from (u) ((edges_of (u) (processed)))) X_low_level_spec )) ,
   (IntArray.full vis1 n vis1_m )
+  **  (((radj + (u * sizeof(PTR) ) )) # Ptr  |-> head)
   **  (SllPtrArray.missing_i radj n u head radj_rows_low_level_spec )
   **  (sllseg head cur processed )
   **  ((&((cur)  # "list" ->ₛ "data")) # Int  |-> vdata)
@@ -500,6 +516,7 @@ forall (n_pre: Z) (radj_rows_low_level_spec: (@list (@list Z))) (X_low_level_spe
 Definition dfs1_entail_wit_3_split_goal_4 := 
 forall (n_pre: Z) (radj_rows_low_level_spec: (@list (@list Z))) (X_low_level_spec: (unit -> (KSt -> Prop))) (g_low_level_spec: AdjGraph) (head: Z) (processed: (@list Z)) (rem: (@list Z)) (vis1_m: (@list Z)) (fin_m: (@list Z)) (timer_m: Z) (vdata: Z) (rest: (@list Z)) (next_ptr: Z) (cur: Z) (n: Z) (u: Z) (radj: Z) (vis1: Z) (fin: Z) (timer_p: Z) (PreH1 : (vdata <= INT_MAX)) (PreH2 : (vdata >= INT_MIN)) (PreH3 : ((Znth vdata vis1_m 0) = 0)) (PreH4 : (cur <> 0)) (PreH5 : (0 <= vdata)) (PreH6 : (vdata < n)) (PreH7 : (n <= INT_MAX)) (PreH8 : (rem = (cons (vdata) (rest)))) (PreH9 : (safeExec (pre_dfs1 (g_low_level_spec) (vis1_m) (fin_m) (timer_m)) (dfs_finish_from (u) ((edges_of (u) (processed)))) X_low_level_spec )) ,
   (IntArray.full vis1 n vis1_m )
+  **  (((radj + (u * sizeof(PTR) ) )) # Ptr  |-> head)
   **  (SllPtrArray.missing_i radj n u head radj_rows_low_level_spec )
   **  (sllseg head cur processed )
   **  ((&((cur)  # "list" ->ₛ "data")) # Int  |-> vdata)
@@ -514,6 +531,7 @@ forall (n_pre: Z) (radj_rows_low_level_spec: (@list (@list Z))) (X_low_level_spe
 Definition dfs1_entail_wit_3_split_goal_5 := 
 forall (n_pre: Z) (u_pre: Z) (radj_rows_low_level_spec: (@list (@list Z))) (X_low_level_spec: (unit -> (KSt -> Prop))) (g_low_level_spec: AdjGraph) (head: Z) (processed: (@list Z)) (rem: (@list Z)) (vis1_m: (@list Z)) (fin_m: (@list Z)) (timer_m: Z) (vdata: Z) (rest: (@list Z)) (next_ptr: Z) (cur: Z) (n: Z) (u: Z) (radj: Z) (vis1: Z) (fin: Z) (timer_p: Z) (PreH1 : (vdata <= INT_MAX)) (PreH2 : (vdata >= INT_MIN)) (PreH3 : ((Znth vdata vis1_m 0) = 0)) (PreH4 : (cur <> 0)) (PreH5 : (0 <= vdata)) (PreH6 : (vdata < n)) (PreH7 : (n <= INT_MAX)) (PreH8 : (rem = (cons (vdata) (rest)))) (PreH9 : (safeExec (pre_dfs1 (g_low_level_spec) (vis1_m) (fin_m) (timer_m)) (dfs_finish_from (u) ((edges_of (u) (processed)))) X_low_level_spec )) ,
   (IntArray.full vis1 n vis1_m )
+  **  (((radj + (u * sizeof(PTR) ) )) # Ptr  |-> head)
   **  (SllPtrArray.missing_i radj n u head radj_rows_low_level_spec )
   **  (sllseg head cur processed )
   **  ((&((cur)  # "list" ->ₛ "data")) # Int  |-> vdata)
@@ -528,6 +546,7 @@ forall (n_pre: Z) (u_pre: Z) (radj_rows_low_level_spec: (@list (@list Z))) (X_lo
 Definition dfs1_entail_wit_3_split_goal_6 := 
 forall (u_pre: Z) (radj_rows_low_level_spec: (@list (@list Z))) (X_low_level_spec: (unit -> (KSt -> Prop))) (g_low_level_spec: AdjGraph) (head: Z) (processed: (@list Z)) (rem: (@list Z)) (vis1_m: (@list Z)) (fin_m: (@list Z)) (timer_m: Z) (vdata: Z) (rest: (@list Z)) (next_ptr: Z) (cur: Z) (n: Z) (u: Z) (radj: Z) (vis1: Z) (fin: Z) (timer_p: Z) (PreH1 : (vdata <= INT_MAX)) (PreH2 : (vdata >= INT_MIN)) (PreH3 : ((Znth vdata vis1_m 0) = 0)) (PreH4 : (cur <> 0)) (PreH5 : (0 <= vdata)) (PreH6 : (vdata < n)) (PreH7 : (n <= INT_MAX)) (PreH8 : (rem = (cons (vdata) (rest)))) (PreH9 : (safeExec (pre_dfs1 (g_low_level_spec) (vis1_m) (fin_m) (timer_m)) (dfs_finish_from (u) ((edges_of (u) (processed)))) X_low_level_spec )) ,
   (IntArray.full vis1 n vis1_m )
+  **  (((radj + (u * sizeof(PTR) ) )) # Ptr  |-> head)
   **  (SllPtrArray.missing_i radj n u head radj_rows_low_level_spec )
   **  (sllseg head cur processed )
   **  ((&((cur)  # "list" ->ₛ "data")) # Int  |-> vdata)
@@ -542,6 +561,7 @@ forall (u_pre: Z) (radj_rows_low_level_spec: (@list (@list Z))) (X_low_level_spe
 Definition dfs1_entail_wit_3_split_goal_7 := 
 forall (n_pre: Z) (radj_rows_low_level_spec: (@list (@list Z))) (X_low_level_spec: (unit -> (KSt -> Prop))) (g_low_level_spec: AdjGraph) (head: Z) (processed: (@list Z)) (rem: (@list Z)) (vis1_m: (@list Z)) (fin_m: (@list Z)) (timer_m: Z) (vdata: Z) (rest: (@list Z)) (next_ptr: Z) (cur: Z) (n: Z) (u: Z) (radj: Z) (vis1: Z) (fin: Z) (timer_p: Z) (PreH1 : (vdata <= INT_MAX)) (PreH2 : (vdata >= INT_MIN)) (PreH3 : ((Znth vdata vis1_m 0) = 0)) (PreH4 : (cur <> 0)) (PreH5 : (0 <= vdata)) (PreH6 : (vdata < n)) (PreH7 : (n <= INT_MAX)) (PreH8 : (rem = (cons (vdata) (rest)))) (PreH9 : (safeExec (pre_dfs1 (g_low_level_spec) (vis1_m) (fin_m) (timer_m)) (dfs_finish_from (u) ((edges_of (u) (processed)))) X_low_level_spec )) ,
   (IntArray.full vis1 n vis1_m )
+  **  (((radj + (u * sizeof(PTR) ) )) # Ptr  |-> head)
   **  (SllPtrArray.missing_i radj n u head radj_rows_low_level_spec )
   **  (sllseg head cur processed )
   **  ((&((cur)  # "list" ->ₛ "data")) # Int  |-> vdata)
@@ -556,6 +576,7 @@ forall (n_pre: Z) (radj_rows_low_level_spec: (@list (@list Z))) (X_low_level_spe
 Definition dfs1_entail_wit_3_split_goal_8 := 
 forall (u_pre: Z) (radj_rows_low_level_spec: (@list (@list Z))) (X_low_level_spec: (unit -> (KSt -> Prop))) (g_low_level_spec: AdjGraph) (head: Z) (processed: (@list Z)) (rem: (@list Z)) (vis1_m: (@list Z)) (fin_m: (@list Z)) (timer_m: Z) (vdata: Z) (rest: (@list Z)) (next_ptr: Z) (cur: Z) (n: Z) (u: Z) (radj: Z) (vis1: Z) (fin: Z) (timer_p: Z) (PreH1 : (vdata <= INT_MAX)) (PreH2 : (vdata >= INT_MIN)) (PreH3 : ((Znth vdata vis1_m 0) = 0)) (PreH4 : (cur <> 0)) (PreH5 : (0 <= vdata)) (PreH6 : (vdata < n)) (PreH7 : (n <= INT_MAX)) (PreH8 : (rem = (cons (vdata) (rest)))) (PreH9 : (safeExec (pre_dfs1 (g_low_level_spec) (vis1_m) (fin_m) (timer_m)) (dfs_finish_from (u) ((edges_of (u) (processed)))) X_low_level_spec )) ,
   (IntArray.full vis1 n vis1_m )
+  **  (((radj + (u * sizeof(PTR) ) )) # Ptr  |-> head)
   **  (SllPtrArray.missing_i radj n u head radj_rows_low_level_spec )
   **  (sllseg head cur processed )
   **  ((&((cur)  # "list" ->ₛ "data")) # Int  |-> vdata)
@@ -570,6 +591,7 @@ forall (u_pre: Z) (radj_rows_low_level_spec: (@list (@list Z))) (X_low_level_spe
 Definition dfs1_entail_wit_3_split_goal_9 := 
 forall (radj_pre: Z) (radj_rows_low_level_spec: (@list (@list Z))) (X_low_level_spec: (unit -> (KSt -> Prop))) (g_low_level_spec: AdjGraph) (head: Z) (processed: (@list Z)) (rem: (@list Z)) (vis1_m: (@list Z)) (fin_m: (@list Z)) (timer_m: Z) (vdata: Z) (rest: (@list Z)) (next_ptr: Z) (cur: Z) (n: Z) (u: Z) (radj: Z) (vis1: Z) (fin: Z) (timer_p: Z) (PreH1 : (vdata <= INT_MAX)) (PreH2 : (vdata >= INT_MIN)) (PreH3 : ((Znth vdata vis1_m 0) = 0)) (PreH4 : (cur <> 0)) (PreH5 : (0 <= vdata)) (PreH6 : (vdata < n)) (PreH7 : (n <= INT_MAX)) (PreH8 : (rem = (cons (vdata) (rest)))) (PreH9 : (safeExec (pre_dfs1 (g_low_level_spec) (vis1_m) (fin_m) (timer_m)) (dfs_finish_from (u) ((edges_of (u) (processed)))) X_low_level_spec )) ,
   (IntArray.full vis1 n vis1_m )
+  **  (((radj + (u * sizeof(PTR) ) )) # Ptr  |-> head)
   **  (SllPtrArray.missing_i radj n u head radj_rows_low_level_spec )
   **  (sllseg head cur processed )
   **  ((&((cur)  # "list" ->ₛ "data")) # Int  |-> vdata)
@@ -584,6 +606,7 @@ forall (radj_pre: Z) (radj_rows_low_level_spec: (@list (@list Z))) (X_low_level_
 Definition dfs1_entail_wit_3_split_goal_10 := 
 forall (vis1_pre: Z) (radj_rows_low_level_spec: (@list (@list Z))) (X_low_level_spec: (unit -> (KSt -> Prop))) (g_low_level_spec: AdjGraph) (head: Z) (processed: (@list Z)) (rem: (@list Z)) (vis1_m: (@list Z)) (fin_m: (@list Z)) (timer_m: Z) (vdata: Z) (rest: (@list Z)) (next_ptr: Z) (cur: Z) (n: Z) (u: Z) (radj: Z) (vis1: Z) (fin: Z) (timer_p: Z) (PreH1 : (vdata <= INT_MAX)) (PreH2 : (vdata >= INT_MIN)) (PreH3 : ((Znth vdata vis1_m 0) = 0)) (PreH4 : (cur <> 0)) (PreH5 : (0 <= vdata)) (PreH6 : (vdata < n)) (PreH7 : (n <= INT_MAX)) (PreH8 : (rem = (cons (vdata) (rest)))) (PreH9 : (safeExec (pre_dfs1 (g_low_level_spec) (vis1_m) (fin_m) (timer_m)) (dfs_finish_from (u) ((edges_of (u) (processed)))) X_low_level_spec )) ,
   (IntArray.full vis1 n vis1_m )
+  **  (((radj + (u * sizeof(PTR) ) )) # Ptr  |-> head)
   **  (SllPtrArray.missing_i radj n u head radj_rows_low_level_spec )
   **  (sllseg head cur processed )
   **  ((&((cur)  # "list" ->ₛ "data")) # Int  |-> vdata)
@@ -598,6 +621,7 @@ forall (vis1_pre: Z) (radj_rows_low_level_spec: (@list (@list Z))) (X_low_level_
 Definition dfs1_entail_wit_3_split_goal_11 := 
 forall (fin_pre: Z) (radj_rows_low_level_spec: (@list (@list Z))) (X_low_level_spec: (unit -> (KSt -> Prop))) (g_low_level_spec: AdjGraph) (head: Z) (processed: (@list Z)) (rem: (@list Z)) (vis1_m: (@list Z)) (fin_m: (@list Z)) (timer_m: Z) (vdata: Z) (rest: (@list Z)) (next_ptr: Z) (cur: Z) (n: Z) (u: Z) (radj: Z) (vis1: Z) (fin: Z) (timer_p: Z) (PreH1 : (vdata <= INT_MAX)) (PreH2 : (vdata >= INT_MIN)) (PreH3 : ((Znth vdata vis1_m 0) = 0)) (PreH4 : (cur <> 0)) (PreH5 : (0 <= vdata)) (PreH6 : (vdata < n)) (PreH7 : (n <= INT_MAX)) (PreH8 : (rem = (cons (vdata) (rest)))) (PreH9 : (safeExec (pre_dfs1 (g_low_level_spec) (vis1_m) (fin_m) (timer_m)) (dfs_finish_from (u) ((edges_of (u) (processed)))) X_low_level_spec )) ,
   (IntArray.full vis1 n vis1_m )
+  **  (((radj + (u * sizeof(PTR) ) )) # Ptr  |-> head)
   **  (SllPtrArray.missing_i radj n u head radj_rows_low_level_spec )
   **  (sllseg head cur processed )
   **  ((&((cur)  # "list" ->ₛ "data")) # Int  |-> vdata)
@@ -612,6 +636,7 @@ forall (fin_pre: Z) (radj_rows_low_level_spec: (@list (@list Z))) (X_low_level_s
 Definition dfs1_entail_wit_3_split_goal_12 := 
 forall (timer_p_pre: Z) (radj_rows_low_level_spec: (@list (@list Z))) (X_low_level_spec: (unit -> (KSt -> Prop))) (g_low_level_spec: AdjGraph) (head: Z) (processed: (@list Z)) (rem: (@list Z)) (vis1_m: (@list Z)) (fin_m: (@list Z)) (timer_m: Z) (vdata: Z) (rest: (@list Z)) (next_ptr: Z) (cur: Z) (n: Z) (u: Z) (radj: Z) (vis1: Z) (fin: Z) (timer_p: Z) (PreH1 : (vdata <= INT_MAX)) (PreH2 : (vdata >= INT_MIN)) (PreH3 : ((Znth vdata vis1_m 0) = 0)) (PreH4 : (cur <> 0)) (PreH5 : (0 <= vdata)) (PreH6 : (vdata < n)) (PreH7 : (n <= INT_MAX)) (PreH8 : (rem = (cons (vdata) (rest)))) (PreH9 : (safeExec (pre_dfs1 (g_low_level_spec) (vis1_m) (fin_m) (timer_m)) (dfs_finish_from (u) ((edges_of (u) (processed)))) X_low_level_spec )) ,
   (IntArray.full vis1 n vis1_m )
+  **  (((radj + (u * sizeof(PTR) ) )) # Ptr  |-> head)
   **  (SllPtrArray.missing_i radj n u head radj_rows_low_level_spec )
   **  (sllseg head cur processed )
   **  ((&((cur)  # "list" ->ₛ "data")) # Int  |-> vdata)
@@ -626,6 +651,7 @@ forall (timer_p_pre: Z) (radj_rows_low_level_spec: (@list (@list Z))) (X_low_lev
 Definition dfs1_entail_wit_3_split_goal_spatial := 
 forall (timer_p_pre: Z) (fin_pre: Z) (vis1_pre: Z) (radj_pre: Z) (n_pre: Z) (radj_rows_low_level_spec: (@list (@list Z))) (X_low_level_spec: (unit -> (KSt -> Prop))) (g_low_level_spec: AdjGraph) (head: Z) (processed: (@list Z)) (rem: (@list Z)) (vis1_m: (@list Z)) (fin_m: (@list Z)) (timer_m: Z) (vdata: Z) (rest: (@list Z)) (next_ptr: Z) (cur: Z) (n: Z) (u: Z) (radj: Z) (vis1: Z) (fin: Z) (timer_p: Z) (PreH1 : (vdata <= INT_MAX)) (PreH2 : (vdata >= INT_MIN)) (PreH3 : ((Znth vdata vis1_m 0) = 0)) (PreH4 : (cur <> 0)) (PreH5 : (0 <= vdata)) (PreH6 : (vdata < n)) (PreH7 : (n <= INT_MAX)) (PreH8 : (rem = (cons (vdata) (rest)))) (PreH9 : (safeExec (pre_dfs1 (g_low_level_spec) (vis1_m) (fin_m) (timer_m)) (dfs_finish_from (u) ((edges_of (u) (processed)))) X_low_level_spec )) ,
   (IntArray.full vis1 n vis1_m )
+  **  (((radj + (u * sizeof(PTR) ) )) # Ptr  |-> head)
   **  (SllPtrArray.missing_i radj n u head radj_rows_low_level_spec )
   **  (sllseg head cur processed )
   **  ((&((cur)  # "list" ->ₛ "data")) # Int  |-> vdata)
@@ -647,6 +673,7 @@ forall (timer_p_pre: Z) (fin_pre: Z) (vis1_pre: Z) (radj_pre: Z) (n_pre: Z) (u_p
   **  ((( &( "n" ) )) # Int  |-> n)
   **  ((( &( "u" ) )) # Int  |-> u)
   **  ((( &( "radj" ) )) # Ptr  |-> radj)
+  **  (((radj + (u * sizeof(PTR) ) )) # Ptr  |-> head)
   **  (SllPtrArray.missing_i radj n u head radj_rows_low_level_spec )
   **  (sllseg head cur processed )
   **  ((&((cur)  # "list" ->ₛ "data")) # Int  |-> vdata)
@@ -671,6 +698,7 @@ forall (timer_p_pre: Z) (fin_pre: Z) (vis1_pre: Z) (radj_pre: Z) (n_pre: Z) (u_p
   **  ((( &( "vis1" ) )) # Ptr  |-> vis1_pre)
   **  ((( &( "fin" ) )) # Ptr  |-> fin_pre)
   **  ((( &( "timer_p" ) )) # Ptr  |-> timer_p_pre)
+  **  (((radj_pre + (u_pre * sizeof(PTR) ) )) # Ptr  |-> head)
   **  (SllPtrArray.missing_i radj_pre n_pre u_pre head radj_rows_low_level_spec )
   **  (sllseg head cur processed )
   **  ((&((cur)  # "list" ->ₛ "data")) # Int  |-> vdata)
@@ -683,6 +711,7 @@ forall (timer_p_pre: Z) (fin_pre: Z) (vis1_pre: Z) (radj_pre: Z) (n_pre: Z) (u_p
 (
 forall (timer_p_pre: Z) (fin_pre: Z) (vis1_pre: Z) (radj_pre: Z) (n_pre: Z) (u_pre: Z) (radj_rows_low_level_spec: (@list (@list Z))) (X_low_level_spec: (unit -> (KSt -> Prop))) (g_low_level_spec: AdjGraph) (head: Z) (processed: (@list Z)) (rem: (@list Z)) (vis1_m: (@list Z)) (fin_m: (@list Z)) (timer_m: Z) (vdata: Z) (rest: (@list Z)) (cur: Z) (n: Z) (u: Z) (radj: Z) (vis1: Z) (fin: Z) (timer_p: Z) (PreH1 : ((Znth vdata vis1_m 0) <> 0)) (PreH2 : (cur <> 0)) (PreH3 : (0 <= vdata)) (PreH4 : (vdata < n)) (PreH5 : (n <= INT_MAX)) (PreH6 : (rem = (cons (vdata) (rest)))) (PreH7 : (safeExec (pre_dfs1 (g_low_level_spec) (vis1_m) (fin_m) (timer_m)) (dfs_finish_from (u) ((edges_of (u) (processed)))) X_low_level_spec )) ,
   (IntArray.full vis1 n vis1_m )
+  **  (((radj + (u * sizeof(PTR) ) )) # Ptr  |-> head)
   **  (SllPtrArray.missing_i radj n u head radj_rows_low_level_spec )
   **  (sllseg head cur processed )
   **  (IntArray.full fin n fin_m )
@@ -701,7 +730,8 @@ forall (timer_p_pre: Z) (fin_pre: Z) (vis1_pre: Z) (radj_pre: Z) (n_pre: Z) (u_p
   &&  “ (n_pre <= INT_MAX) ” 
   &&  “ (rem = (cons (vdata) (rest))) ” 
   &&  “ (safeExec (pre_dfs1 (g_low_level_spec) (vis1_m_) (fin_m_) (timer_m_)) (dfs_finish_from (u_pre) ((edges_of (u_pre) (processed)))) X_low_level_spec ) ”
-  &&  (SllPtrArray.missing_i radj_pre n_pre u_pre head radj_rows_low_level_spec )
+  &&  (((radj_pre + (u_pre * sizeof(PTR) ) )) # Ptr  |-> head)
+  **  (SllPtrArray.missing_i radj_pre n_pre u_pre head radj_rows_low_level_spec )
   **  (sllseg head cur processed )
   **  (IntArray.full vis1_pre n_pre vis1_m_ )
   **  (IntArray.full fin_pre n_pre fin_m_ )
@@ -723,7 +753,8 @@ forall (timer_p_pre: Z) (fin_pre: Z) (vis1_pre: Z) (radj_pre: Z) (n_pre: Z) (u_p
   &&  “ (n_pre <= INT_MAX) ” 
   &&  “ (rem = (cons (v) (rest_))) ” 
   &&  “ (safeExec (pre_dfs1 (g_low_level_spec) (vis1_m_) (fin_m_) (timer_m_)) (dfs_finish_from (u_pre) ((edges_of (u_pre) (processed)))) X_low_level_spec ) ”
-  &&  (SllPtrArray.missing_i radj_pre n_pre u_pre head radj_rows_low_level_spec )
+  &&  (((radj_pre + (u_pre * sizeof(PTR) ) )) # Ptr  |-> head)
+  **  (SllPtrArray.missing_i radj_pre n_pre u_pre head radj_rows_low_level_spec )
   **  (sllseg head cur processed )
   **  ((&((cur)  # "list" ->ₛ "data")) # Int  |-> v)
   **  ((&((cur)  # "list" ->ₛ "next")) # Ptr  |-> next_ptr_)
@@ -733,11 +764,13 @@ forall (timer_p_pre: Z) (fin_pre: Z) (vis1_pre: Z) (radj_pre: Z) (n_pre: Z) (u_p
   **  (IntArray.full timer_p_pre 1 (cons (timer_m_) ((@nil Z))) )
 ) \/
 (
-forall (radj_pre: Z) (n_pre: Z) (u_pre: Z) (radj_rows_low_level_spec: (@list (@list Z))) (X_low_level_spec: (unit -> (KSt -> Prop))) (g_low_level_spec: AdjGraph) (head: Z) (processed: (@list Z)) (rem: (@list Z)) (vis1_m: (@list Z)) (cur: Z) (v: Z) (vis1_l_: (@list Z)) (fin_l_: (@list Z)) (timer_v_: Z) (PreH1 : (safeExec (pre_dfs1 (g_low_level_spec) (vis1_l_) (fin_l_) (timer_v_)) (return (tt)) X_low_level_spec )) (PreH2 : (cur <> 0)) (PreH3 : (0 <= u_pre)) (PreH4 : (u_pre < n_pre)) (PreH5 : (0 <= v)) (PreH6 : (v < n_pre)) (PreH7 : (n_pre <= INT_MAX)) (PreH8 : ((Znth (v) (vis1_m) (0)) = 0)) ,
-  (SllPtrArray.full radj_pre n_pre radj_rows_low_level_spec )
+forall (radj_pre: Z) (n_pre: Z) (u_pre: Z) (radj_rows_low_level_spec: (@list (@list Z))) (X_low_level_spec: (unit -> (KSt -> Prop))) (g_low_level_spec: AdjGraph) (head: Z) (processed: (@list Z)) (rem: (@list Z)) (vis1_m: (@list Z)) (cur: Z) (v: Z) (vis1_l_: (@list Z)) (fin_l_: (@list Z)) (timer_v_: Z) (row_ptr: Z)  __default__List_Z (PreH1 : (safeExec (pre_dfs1 (g_low_level_spec) (vis1_l_) (fin_l_) (timer_v_)) (return (tt)) X_low_level_spec )) (PreH2 : (cur <> 0)) (PreH3 : (0 <= u_pre)) (PreH4 : (u_pre < n_pre)) (PreH5 : (0 <= v)) (PreH6 : (v < n_pre)) (PreH7 : (n_pre <= INT_MAX)) (PreH8 : ((Znth (v) (vis1_m) (0)) = 0)) ,
+  (sll row_ptr (Znth u_pre radj_rows_low_level_spec __default__List_Z) )
+  **  (SllPtrArray.missing_i radj_pre n_pre u_pre row_ptr radj_rows_low_level_spec )
 |--
   EX (next_ptr_: Z)  (timer_m_: Z)  (rest_: (@list Z)) ,
-  “ ((cons (timer_v_) ((@nil Z))) = (cons (timer_m_) ((@nil Z)))) ” 
+  “ (head = row_ptr) ” 
+  &&  “ ((cons (timer_v_) ((@nil Z))) = (cons (timer_m_) ((@nil Z)))) ” 
   &&  “ (cur <> 0) ” 
   &&  “ (0 <= u_pre) ” 
   &&  “ (u_pre < n_pre) ” 
@@ -754,7 +787,8 @@ forall (radj_pre: Z) (n_pre: Z) (u_pre: Z) (radj_rows_low_level_spec: (@list (@l
 Definition dfs1_entail_wit_5 := 
 (
 forall (timer_p_pre: Z) (fin_pre: Z) (vis1_pre: Z) (radj_pre: Z) (n_pre: Z) (u_pre: Z) (radj_rows_low_level_spec: (@list (@list Z))) (X_low_level_spec: (unit -> (KSt -> Prop))) (g_low_level_spec: AdjGraph) (head_2: Z) (processed_2: (@list Z)) (rem_2: (@list Z)) (vdata_: Z) (rest_: (@list Z)) (next_ptr_: Z) (vis1_m_: (@list Z)) (fin_m_: (@list Z)) (timer_m_: Z) (cur: Z) (PreH1 : (cur <> 0)) (PreH2 : (0 <= u_pre)) (PreH3 : (u_pre < n_pre)) (PreH4 : (n_pre <= INT_MAX)) (PreH5 : (rem_2 = (cons (vdata_) (rest_)))) (PreH6 : (safeExec (pre_dfs1 (g_low_level_spec) (vis1_m_) (fin_m_) (timer_m_)) (dfs_finish_from (u_pre) ((edges_of (u_pre) (processed_2)))) X_low_level_spec )) ,
-  (SllPtrArray.missing_i radj_pre n_pre u_pre head_2 radj_rows_low_level_spec )
+  (((radj_pre + (u_pre * sizeof(PTR) ) )) # Ptr  |-> head_2)
+  **  (SllPtrArray.missing_i radj_pre n_pre u_pre head_2 radj_rows_low_level_spec )
   **  (sllseg head_2 cur processed_2 )
   **  ((&((cur)  # "list" ->ₛ "data")) # Int  |-> vdata_)
   **  ((&((cur)  # "list" ->ₛ "next")) # Ptr  |-> next_ptr_)
@@ -768,7 +802,8 @@ forall (timer_p_pre: Z) (fin_pre: Z) (vis1_pre: Z) (radj_pre: Z) (n_pre: Z) (u_p
   &&  “ (0 <= u_pre) ” 
   &&  “ (u_pre < n_pre) ” 
   &&  “ (n_pre <= INT_MAX) ”
-  &&  (SllPtrArray.missing_i radj_pre n_pre u_pre head radj_rows_low_level_spec )
+  &&  (((radj_pre + (u_pre * sizeof(PTR) ) )) # Ptr  |-> head)
+  **  (SllPtrArray.missing_i radj_pre n_pre u_pre head radj_rows_low_level_spec )
   **  (sllseg head next_ptr_ processed )
   **  (sll next_ptr_ rem )
   **  (IntArray.full vis1_pre n_pre vis1_m )
@@ -776,26 +811,25 @@ forall (timer_p_pre: Z) (fin_pre: Z) (vis1_pre: Z) (radj_pre: Z) (n_pre: Z) (u_p
   **  (IntArray.full timer_p_pre 1 (cons (timer_m) ((@nil Z))) )
 ) \/
 (
-forall (radj_pre: Z) (n_pre: Z) (u_pre: Z) (radj_rows_low_level_spec: (@list (@list Z))) (X_low_level_spec: (unit -> (KSt -> Prop))) (g_low_level_spec: AdjGraph) (head_2: Z) (processed_2: (@list Z)) (rem_2: (@list Z)) (vdata_: Z) (rest_: (@list Z)) (next_ptr_: Z) (vis1_m_: (@list Z)) (fin_m_: (@list Z)) (timer_m_: Z) (cur: Z) (PreH1 : (vdata_ <= INT_MAX)) (PreH2 : (vdata_ >= INT_MIN)) (PreH3 : (cur <> 0)) (PreH4 : (0 <= u_pre)) (PreH5 : (u_pre < n_pre)) (PreH6 : (n_pre <= INT_MAX)) (PreH7 : (rem_2 = (cons (vdata_) (rest_)))) (PreH8 : (safeExec (pre_dfs1 (g_low_level_spec) (vis1_m_) (fin_m_) (timer_m_)) (dfs_finish_from (u_pre) ((edges_of (u_pre) (processed_2)))) X_low_level_spec )) ,
-  (SllPtrArray.missing_i radj_pre n_pre u_pre head_2 radj_rows_low_level_spec )
-  **  (sllseg head_2 cur processed_2 )
+forall (n_pre: Z) (u_pre: Z) (X_low_level_spec: (unit -> (KSt -> Prop))) (g_low_level_spec: AdjGraph) (head_2: Z) (processed_2: (@list Z)) (rem_2: (@list Z)) (vdata_: Z) (rest_: (@list Z)) (next_ptr_: Z) (vis1_m_: (@list Z)) (fin_m_: (@list Z)) (timer_m_: Z) (cur: Z) (PreH1 : (vdata_ <= INT_MAX)) (PreH2 : (vdata_ >= INT_MIN)) (PreH3 : (cur <> 0)) (PreH4 : (0 <= u_pre)) (PreH5 : (u_pre < n_pre)) (PreH6 : (n_pre <= INT_MAX)) (PreH7 : (rem_2 = (cons (vdata_) (rest_)))) (PreH8 : (safeExec (pre_dfs1 (g_low_level_spec) (vis1_m_) (fin_m_) (timer_m_)) (dfs_finish_from (u_pre) ((edges_of (u_pre) (processed_2)))) X_low_level_spec )) ,
+  (sllseg head_2 cur processed_2 )
   **  ((&((cur)  # "list" ->ₛ "data")) # Int  |-> vdata_)
   **  ((&((cur)  # "list" ->ₛ "next")) # Ptr  |-> next_ptr_)
 |--
-  EX (head: Z)  (timer_m: Z)  (processed: (@list Z)) ,
+  EX (timer_m: Z)  (processed: (@list Z)) ,
   “ ((cons (timer_m_) ((@nil Z))) = (cons (timer_m) ((@nil Z)))) ” 
   &&  “ (safeExec (pre_dfs1 (g_low_level_spec) (vis1_m_) (fin_m_) (timer_m)) (dfs_finish_from (u_pre) ((edges_of (u_pre) (processed)))) X_low_level_spec ) ” 
   &&  “ (0 <= u_pre) ” 
   &&  “ (u_pre < n_pre) ” 
   &&  “ (n_pre <= INT_MAX) ”
-  &&  (SllPtrArray.missing_i radj_pre n_pre u_pre head radj_rows_low_level_spec )
-  **  (sllseg head next_ptr_ processed )
+  &&  (sllseg head_2 next_ptr_ processed )
 ).
 
 Definition dfs1_entail_wit_6 := 
 (
 forall (timer_p_pre: Z) (fin_pre: Z) (vis1_pre: Z) (radj_pre: Z) (n_pre: Z) (u_pre: Z) (radj_rows_low_level_spec: (@list (@list Z))) (X_low_level_spec: (unit -> (KSt -> Prop))) (g_low_level_spec: AdjGraph) (rem: (@list Z)) (cur: Z) (head_2: Z) (vis1_m_2: (@list Z)) (fin_m_2: (@list Z)) (timer_m: Z) (processed: (@list Z)) (PreH1 : (cur = 0)) (PreH2 : (safeExec (pre_dfs1 (g_low_level_spec) (vis1_m_2) (fin_m_2) (timer_m)) (dfs_finish_from (u_pre) ((edges_of (u_pre) (processed)))) X_low_level_spec )) (PreH3 : (0 <= u_pre)) (PreH4 : (u_pre < n_pre)) (PreH5 : (n_pre <= INT_MAX)) ,
   (IntArray.full timer_p_pre 1 (cons (timer_m) ((@nil Z))) )
+  **  (((radj_pre + (u_pre * sizeof(PTR) ) )) # Ptr  |-> head_2)
   **  (SllPtrArray.missing_i radj_pre n_pre u_pre head_2 radj_rows_low_level_spec )
   **  ((( &( "cur" ) )) # Ptr  |-> cur)
   **  (sllseg head_2 cur processed )
@@ -810,7 +844,8 @@ forall (timer_p_pre: Z) (fin_pre: Z) (vis1_pre: Z) (radj_pre: Z) (n_pre: Z) (u_p
   &&  “ (fin_m_set = (replace_Znth (u_pre) ((Znth 0 (cons (timer_m) ((@nil Z))) 0)) (fin_m))) ” 
   &&  “ (timer_m_set = ((Znth 0 (cons (timer_m) ((@nil Z))) 0) + 1 )) ” 
   &&  “ (safeExec (pre_dfs1 (g_low_level_spec) (vis1_m) (fin_m_set) (timer_m_set)) (return (tt)) X_low_level_spec ) ”
-  &&  (SllPtrArray.missing_i radj_pre n_pre u_pre head radj_rows_low_level_spec )
+  &&  (((radj_pre + (u_pre * sizeof(PTR) ) )) # Ptr  |-> head)
+  **  (SllPtrArray.missing_i radj_pre n_pre u_pre head radj_rows_low_level_spec )
   **  (sll head (Znth (u_pre) (radj_rows_low_level_spec) ((@nil Z))) )
   **  ((( &( "cur" ) )) # Ptr  |-> 0)
   **  (IntArray.full vis1_pre n_pre vis1_m )
@@ -818,12 +853,11 @@ forall (timer_p_pre: Z) (fin_pre: Z) (vis1_pre: Z) (radj_pre: Z) (n_pre: Z) (u_p
   **  (IntArray.full timer_p_pre 1 (cons ((Znth 0 (cons (timer_m) ((@nil Z))) 0)) ((@nil Z))) )
 ) \/
 (
-forall (radj_pre: Z) (n_pre: Z) (u_pre: Z) (radj_rows_low_level_spec: (@list (@list Z))) (X_low_level_spec: (unit -> (KSt -> Prop))) (g_low_level_spec: AdjGraph) (rem: (@list Z)) (cur: Z) (head_2: Z) (vis1_m_2: (@list Z)) (fin_m_2: (@list Z)) (timer_m: Z) (processed: (@list Z)) (PreH1 : (cur = 0)) (PreH2 : (safeExec (pre_dfs1 (g_low_level_spec) (vis1_m_2) (fin_m_2) (timer_m)) (dfs_finish_from (u_pre) ((edges_of (u_pre) (processed)))) X_low_level_spec )) (PreH3 : (0 <= u_pre)) (PreH4 : (u_pre < n_pre)) (PreH5 : (n_pre <= INT_MAX)) ,
-  (SllPtrArray.missing_i radj_pre n_pre u_pre head_2 radj_rows_low_level_spec )
-  **  (sllseg head_2 cur processed )
+forall (n_pre: Z) (u_pre: Z) (radj_rows_low_level_spec: (@list (@list Z))) (X_low_level_spec: (unit -> (KSt -> Prop))) (g_low_level_spec: AdjGraph) (rem: (@list Z)) (cur: Z) (head_2: Z) (vis1_m_2: (@list Z)) (fin_m_2: (@list Z)) (timer_m: Z) (processed: (@list Z)) (PreH1 : (cur = 0)) (PreH2 : (safeExec (pre_dfs1 (g_low_level_spec) (vis1_m_2) (fin_m_2) (timer_m)) (dfs_finish_from (u_pre) ((edges_of (u_pre) (processed)))) X_low_level_spec )) (PreH3 : (0 <= u_pre)) (PreH4 : (u_pre < n_pre)) (PreH5 : (n_pre <= INT_MAX)) ,
+  (sllseg head_2 cur processed )
   **  (sll cur rem )
 |--
-  EX (head: Z)  (fin_m: (@list Z)) ,
+  EX (fin_m: (@list Z)) ,
   “ (fin_m_2 = (replace_Znth (u_pre) ((Znth 0 (cons (timer_m) ((@nil Z))) 0)) (fin_m))) ” 
   &&  “ ((cons (timer_m) ((@nil Z))) = (cons ((Znth 0 (cons (timer_m) ((@nil Z))) 0)) ((@nil Z)))) ” 
   &&  “ (cur = 0) ” 
@@ -831,8 +865,7 @@ forall (radj_pre: Z) (n_pre: Z) (u_pre: Z) (radj_rows_low_level_spec: (@list (@l
   &&  “ (u_pre < n_pre) ” 
   &&  “ (n_pre <= INT_MAX) ” 
   &&  “ (safeExec (pre_dfs1 (g_low_level_spec) (vis1_m_2) ((replace_Znth (u_pre) ((Znth 0 (cons (timer_m) ((@nil Z))) 0)) (fin_m))) (((Znth 0 (cons (timer_m) ((@nil Z))) 0) + 1 ))) (return (tt)) X_low_level_spec ) ”
-  &&  (SllPtrArray.missing_i radj_pre n_pre u_pre head radj_rows_low_level_spec )
-  **  (sll head (Znth (u_pre) (radj_rows_low_level_spec) ((@nil Z))) )
+  &&  (sll head_2 (Znth (u_pre) (radj_rows_low_level_spec) ((@nil Z))) )
 ).
 
 Definition dfs1_return_wit_1 := 
@@ -840,6 +873,7 @@ Definition dfs1_return_wit_1 :=
 forall (timer_p_pre: Z) (fin_pre: Z) (vis1_pre: Z) (radj_pre: Z) (n_pre: Z) (u_pre: Z) (radj_rows_low_level_spec: (@list (@list Z))) (X_low_level_spec: (unit -> (KSt -> Prop))) (g_low_level_spec: AdjGraph) (head: Z) (vis1_m: (@list Z)) (fin_m: (@list Z)) (timer_m: Z) (fin_m_set: (@list Z)) (timer_m_set: Z) (PreH1 : (0 <= u_pre)) (PreH2 : (u_pre < n_pre)) (PreH3 : (n_pre <= INT_MAX)) (PreH4 : (fin_m_set = (replace_Znth (u_pre) (timer_m) (fin_m)))) (PreH5 : (timer_m_set = (timer_m + 1 ))) (PreH6 : (safeExec (pre_dfs1 (g_low_level_spec) (vis1_m) (fin_m_set) (timer_m_set)) (return (tt)) X_low_level_spec )) ,
   (IntArray.full timer_p_pre 1 (replace_Znth (0) ((timer_m + 1 )) ((cons (timer_m) ((@nil Z))))) )
   **  (IntArray.full fin_pre n_pre (replace_Znth (u_pre) (timer_m) (fin_m_set)) )
+  **  (((radj_pre + (u_pre * sizeof(PTR) ) )) # Ptr  |-> head)
   **  (SllPtrArray.missing_i radj_pre n_pre u_pre head radj_rows_low_level_spec )
   **  (sll head (Znth (u_pre) (radj_rows_low_level_spec) ((@nil Z))) )
   **  (IntArray.full vis1_pre n_pre vis1_m )
@@ -853,7 +887,8 @@ forall (timer_p_pre: Z) (fin_pre: Z) (vis1_pre: Z) (radj_pre: Z) (n_pre: Z) (u_p
 ) \/
 (
 forall (radj_pre: Z) (n_pre: Z) (u_pre: Z) (radj_rows_low_level_spec: (@list (@list Z))) (X_low_level_spec: (unit -> (KSt -> Prop))) (g_low_level_spec: AdjGraph) (head: Z) (vis1_m: (@list Z)) (fin_m: (@list Z)) (timer_m: Z) (fin_m_set: (@list Z)) (timer_m_set: Z) (PreH1 : (0 <= u_pre)) (PreH2 : (u_pre < n_pre)) (PreH3 : (n_pre <= INT_MAX)) (PreH4 : (fin_m_set = (replace_Znth (u_pre) (timer_m) (fin_m)))) (PreH5 : (timer_m_set = (timer_m + 1 ))) (PreH6 : (safeExec (pre_dfs1 (g_low_level_spec) (vis1_m) (fin_m_set) (timer_m_set)) (return (tt)) X_low_level_spec )) ,
-  (SllPtrArray.missing_i radj_pre n_pre u_pre head radj_rows_low_level_spec )
+  (((radj_pre + (u_pre * sizeof(PTR) ) )) # Ptr  |-> head)
+  **  (SllPtrArray.missing_i radj_pre n_pre u_pre head radj_rows_low_level_spec )
   **  (sll head (Znth (u_pre) (radj_rows_low_level_spec) ((@nil Z))) )
 |--
   EX (timer_v_: Z) ,
@@ -902,7 +937,8 @@ forall (timer_p_pre: Z) (fin_pre: Z) (vis1_pre: Z) (radj_pre: Z) (n_pre: Z) (u_p
 
 Definition dfs1_partial_solve_wit_3 := 
 forall (radj_rows_low_level_spec: (@list (@list Z))) (X_low_level_spec: (unit -> (KSt -> Prop))) (g_low_level_spec: AdjGraph) (head: Z) (processed: (@list Z)) (rem: (@list Z)) (vis1_m: (@list Z)) (fin_m: (@list Z)) (timer_m: Z) (vdata: Z) (rest: (@list Z)) (next_ptr: Z) (cur: Z) (n: Z) (u: Z) (radj: Z) (vis1: Z) (fin: Z) (timer_p: Z) (PreH1 : (cur <> 0)) (PreH2 : (0 <= vdata)) (PreH3 : (vdata < n)) (PreH4 : (n <= INT_MAX)) (PreH5 : (rem = (cons (vdata) (rest)))) (PreH6 : (safeExec (pre_dfs1 (g_low_level_spec) (vis1_m) (fin_m) (timer_m)) (dfs_finish_from (u) ((edges_of (u) (processed)))) X_low_level_spec )) ,
-  (SllPtrArray.missing_i radj n u head radj_rows_low_level_spec )
+  (((radj + (u * sizeof(PTR) ) )) # Ptr  |-> head)
+  **  (SllPtrArray.missing_i radj n u head radj_rows_low_level_spec )
   **  (sllseg head cur processed )
   **  ((&((cur)  # "list" ->ₛ "data")) # Int  |-> vdata)
   **  ((&((cur)  # "list" ->ₛ "next")) # Ptr  |-> next_ptr)
@@ -919,6 +955,7 @@ forall (radj_rows_low_level_spec: (@list (@list Z))) (X_low_level_spec: (unit ->
   &&  “ (safeExec (pre_dfs1 (g_low_level_spec) (vis1_m) (fin_m) (timer_m)) (dfs_finish_from (u) ((edges_of (u) (processed)))) X_low_level_spec ) ”
   &&  (((vis1 + (vdata * sizeof(INT) ) )) # Int  |-> (Znth vdata vis1_m 0))
   **  (IntArray.missing_i vis1 vdata 0 n vis1_m )
+  **  (((radj + (u * sizeof(PTR) ) )) # Ptr  |-> head)
   **  (SllPtrArray.missing_i radj n u head radj_rows_low_level_spec )
   **  (sllseg head cur processed )
   **  ((&((cur)  # "list" ->ₛ "data")) # Int  |-> vdata)
@@ -978,7 +1015,8 @@ Definition dfs1_partial_solve_wit_4 := dfs1_partial_solve_wit_4_pure -> dfs1_par
 
 Definition dfs1_partial_solve_wit_5 := 
 forall (timer_p_pre: Z) (fin_pre: Z) (vis1_pre: Z) (radj_pre: Z) (n_pre: Z) (u_pre: Z) (radj_rows_low_level_spec: (@list (@list Z))) (X_low_level_spec: (unit -> (KSt -> Prop))) (g_low_level_spec: AdjGraph) (rem: (@list Z)) (cur: Z) (head: Z) (vis1_m: (@list Z)) (fin_m: (@list Z)) (timer_m: Z) (processed: (@list Z)) (PreH1 : (cur = 0)) (PreH2 : (safeExec (pre_dfs1 (g_low_level_spec) (vis1_m) (fin_m) (timer_m)) (dfs_finish_from (u_pre) ((edges_of (u_pre) (processed)))) X_low_level_spec )) (PreH3 : (0 <= u_pre)) (PreH4 : (u_pre < n_pre)) (PreH5 : (n_pre <= INT_MAX)) ,
-  (SllPtrArray.missing_i radj_pre n_pre u_pre head radj_rows_low_level_spec )
+  (((radj_pre + (u_pre * sizeof(PTR) ) )) # Ptr  |-> head)
+  **  (SllPtrArray.missing_i radj_pre n_pre u_pre head radj_rows_low_level_spec )
   **  (sllseg head cur processed )
   **  (sll cur rem )
   **  (IntArray.full vis1_pre n_pre vis1_m )
@@ -992,6 +1030,7 @@ forall (timer_p_pre: Z) (fin_pre: Z) (vis1_pre: Z) (radj_pre: Z) (n_pre: Z) (u_p
   &&  “ (n_pre <= INT_MAX) ”
   &&  (((timer_p_pre + (0 * sizeof(INT) ) )) # Int  |-> (Znth 0 (cons (timer_m) ((@nil Z))) 0))
   **  (IntArray.missing_i timer_p_pre 0 0 1 (cons (timer_m) ((@nil Z))) )
+  **  (((radj_pre + (u_pre * sizeof(PTR) ) )) # Ptr  |-> head)
   **  (SllPtrArray.missing_i radj_pre n_pre u_pre head radj_rows_low_level_spec )
   **  (sllseg head cur processed )
   **  (sll cur rem )
@@ -1001,7 +1040,8 @@ forall (timer_p_pre: Z) (fin_pre: Z) (vis1_pre: Z) (radj_pre: Z) (n_pre: Z) (u_p
 
 Definition dfs1_partial_solve_wit_6 := 
 forall (timer_p_pre: Z) (fin_pre: Z) (vis1_pre: Z) (radj_pre: Z) (n_pre: Z) (u_pre: Z) (radj_rows_low_level_spec: (@list (@list Z))) (X_low_level_spec: (unit -> (KSt -> Prop))) (g_low_level_spec: AdjGraph) (head: Z) (vis1_m: (@list Z)) (fin_m: (@list Z)) (timer_m: Z) (fin_m_set: (@list Z)) (timer_m_set: Z) (PreH1 : (0 <= u_pre)) (PreH2 : (u_pre < n_pre)) (PreH3 : (n_pre <= INT_MAX)) (PreH4 : (fin_m_set = (replace_Znth (u_pre) (timer_m) (fin_m)))) (PreH5 : (timer_m_set = (timer_m + 1 ))) (PreH6 : (safeExec (pre_dfs1 (g_low_level_spec) (vis1_m) (fin_m_set) (timer_m_set)) (return (tt)) X_low_level_spec )) ,
-  (SllPtrArray.missing_i radj_pre n_pre u_pre head radj_rows_low_level_spec )
+  (((radj_pre + (u_pre * sizeof(PTR) ) )) # Ptr  |-> head)
+  **  (SllPtrArray.missing_i radj_pre n_pre u_pre head radj_rows_low_level_spec )
   **  (sll head (Znth (u_pre) (radj_rows_low_level_spec) ((@nil Z))) )
   **  (IntArray.full vis1_pre n_pre vis1_m )
   **  (IntArray.full fin_pre n_pre fin_m_set )
@@ -1015,6 +1055,7 @@ forall (timer_p_pre: Z) (fin_pre: Z) (vis1_pre: Z) (radj_pre: Z) (n_pre: Z) (u_p
   &&  “ (safeExec (pre_dfs1 (g_low_level_spec) (vis1_m) (fin_m_set) (timer_m_set)) (return (tt)) X_low_level_spec ) ”
   &&  (((fin_pre + (u_pre * sizeof(INT) ) )) # Int  |->_)
   **  (IntArray.missing_i fin_pre u_pre 0 n_pre fin_m_set )
+  **  (((radj_pre + (u_pre * sizeof(PTR) ) )) # Ptr  |-> head)
   **  (SllPtrArray.missing_i radj_pre n_pre u_pre head radj_rows_low_level_spec )
   **  (sll head (Znth (u_pre) (radj_rows_low_level_spec) ((@nil Z))) )
   **  (IntArray.full vis1_pre n_pre vis1_m )
@@ -1024,6 +1065,7 @@ forall (timer_p_pre: Z) (fin_pre: Z) (vis1_pre: Z) (radj_pre: Z) (n_pre: Z) (u_p
 Definition dfs1_partial_solve_wit_7 := 
 forall (timer_p_pre: Z) (fin_pre: Z) (vis1_pre: Z) (radj_pre: Z) (n_pre: Z) (u_pre: Z) (radj_rows_low_level_spec: (@list (@list Z))) (X_low_level_spec: (unit -> (KSt -> Prop))) (g_low_level_spec: AdjGraph) (head: Z) (vis1_m: (@list Z)) (fin_m: (@list Z)) (timer_m: Z) (fin_m_set: (@list Z)) (timer_m_set: Z) (PreH1 : (0 <= u_pre)) (PreH2 : (u_pre < n_pre)) (PreH3 : (n_pre <= INT_MAX)) (PreH4 : (fin_m_set = (replace_Znth (u_pre) (timer_m) (fin_m)))) (PreH5 : (timer_m_set = (timer_m + 1 ))) (PreH6 : (safeExec (pre_dfs1 (g_low_level_spec) (vis1_m) (fin_m_set) (timer_m_set)) (return (tt)) X_low_level_spec )) ,
   (IntArray.full fin_pre n_pre (replace_Znth (u_pre) (timer_m) (fin_m_set)) )
+  **  (((radj_pre + (u_pre * sizeof(PTR) ) )) # Ptr  |-> head)
   **  (SllPtrArray.missing_i radj_pre n_pre u_pre head radj_rows_low_level_spec )
   **  (sll head (Znth (u_pre) (radj_rows_low_level_spec) ((@nil Z))) )
   **  (IntArray.full vis1_pre n_pre vis1_m )
@@ -1038,6 +1080,7 @@ forall (timer_p_pre: Z) (fin_pre: Z) (vis1_pre: Z) (radj_pre: Z) (n_pre: Z) (u_p
   &&  (((timer_p_pre + (0 * sizeof(INT) ) )) # Int  |->_)
   **  (IntArray.missing_i timer_p_pre 0 0 1 (cons (timer_m) ((@nil Z))) )
   **  (IntArray.full fin_pre n_pre (replace_Znth (u_pre) (timer_m) (fin_m_set)) )
+  **  (((radj_pre + (u_pre * sizeof(PTR) ) )) # Ptr  |-> head)
   **  (SllPtrArray.missing_i radj_pre n_pre u_pre head radj_rows_low_level_spec )
   **  (sll head (Znth (u_pre) (radj_rows_low_level_spec) ((@nil Z))) )
   **  (IntArray.full vis1_pre n_pre vis1_m )
@@ -1069,6 +1112,7 @@ forall (sid_pre: Z) (vis2_pre: Z) (fadj_pre: Z) (n_pre: Z) (u_pre: Z) (root_pre:
   **  ((( &( "fadj" ) )) # Ptr  |-> fadj_pre)
   **  ((( &( "vis2" ) )) # Ptr  |-> vis2_pre)
   **  ((( &( "sid" ) )) # Ptr  |-> sid_pre)
+  **  (((fadj_pre + (u_pre * sizeof(PTR) ) )) # Ptr  |-> head)
   **  (SllPtrArray.missing_i fadj_pre n_pre u_pre head fadj_rows_low_level_spec )
   **  ((( &( "cur" ) )) # Ptr  |-> cur)
   **  (sllseg head cur processed )
@@ -1089,6 +1133,7 @@ forall (fadj_rows_low_level_spec: (@list (@list Z))) (X_low_level_spec: (unit ->
   **  ((( &( "u" ) )) # Int  |-> u)
   **  ((( &( "root" ) )) # Int  |-> root)
   **  ((( &( "fadj" ) )) # Ptr  |-> fadj)
+  **  (((fadj + (u * sizeof(PTR) ) )) # Ptr  |-> head)
   **  (SllPtrArray.missing_i fadj n u head fadj_rows_low_level_spec )
   **  (sllseg head cur processed )
   **  ((&((cur)  # "list" ->ₛ "data")) # Int  |-> vdata)
@@ -1116,25 +1161,25 @@ forall (sid_pre: Z) (vis2_pre: Z) (fadj_pre: Z) (n_pre: Z) (u_pre: Z) (root_pre:
   &&  “ (0 <= u_pre) ” 
   &&  “ (u_pre < n_pre) ” 
   &&  “ (n_pre <= INT_MAX) ”
-  &&  (SllPtrArray.missing_i fadj_pre n_pre u_pre head fadj_rows_low_level_spec )
+  &&  (((fadj_pre + (u_pre * sizeof(PTR) ) )) # Ptr  |-> head)
+  **  (SllPtrArray.missing_i fadj_pre n_pre u_pre head fadj_rows_low_level_spec )
   **  (sllseg head row_ptr processed )
   **  (sll row_ptr rem )
   **  (IntArray.full vis2_pre n_pre vis2_m )
   **  (IntArray.full sid_pre n_pre sid_m )
 ) \/
 (
-forall (fadj_pre: Z) (n_pre: Z) (u_pre: Z) (root_pre: Z) (fadj_rows_low_level_spec: (@list (@list Z))) (X_low_level_spec: (unit -> (KSt -> Prop))) (sid_l_low_level_spec: (@list Z)) (vis2_l_low_level_spec: (@list Z)) (g_low_level_spec: AdjGraph) (row_ptr: Z) (PreH1 : (safeExec (pre_dfs2 (g_low_level_spec) (vis2_l_low_level_spec) (sid_l_low_level_spec)) (dfs_scc (root_pre) (u_pre)) X_low_level_spec )) (PreH2 : (0 <= root_pre)) (PreH3 : (root_pre < n_pre)) (PreH4 : (0 <= u_pre)) (PreH5 : (u_pre < n_pre)) (PreH6 : (n_pre <= INT_MAX)) ,
-  (SllPtrArray.full fadj_pre n_pre fadj_rows_low_level_spec )
+forall (n_pre: Z) (u_pre: Z) (root_pre: Z) (fadj_rows_low_level_spec: (@list (@list Z))) (X_low_level_spec: (unit -> (KSt -> Prop))) (sid_l_low_level_spec: (@list Z)) (vis2_l_low_level_spec: (@list Z)) (g_low_level_spec: AdjGraph) (row_ptr: Z) (row_ptr_2: Z)  __default__List_Z (PreH1 : (safeExec (pre_dfs2 (g_low_level_spec) (vis2_l_low_level_spec) (sid_l_low_level_spec)) (dfs_scc (root_pre) (u_pre)) X_low_level_spec )) (PreH2 : (0 <= root_pre)) (PreH3 : (root_pre < n_pre)) (PreH4 : (0 <= u_pre)) (PreH5 : (u_pre < n_pre)) (PreH6 : (n_pre <= INT_MAX)) ,
+  (sll row_ptr_2 (Znth u_pre fadj_rows_low_level_spec __default__List_Z) )
 |--
-  EX (rem: (@list Z))  (head: Z)  (processed: (@list Z)) ,
+  EX (rem: (@list Z))  (processed: (@list Z)) ,
   “ (safeExec (pre_dfs2 (g_low_level_spec) ((replace_Znth (u_pre) (1) (vis2_l_low_level_spec))) ((replace_Znth (u_pre) ((Znth root_pre sid_l_low_level_spec 0)) (sid_l_low_level_spec)))) (dfs_scc_from (root_pre) (u_pre) ((edges_of (u_pre) (processed)))) X_low_level_spec ) ” 
   &&  “ (0 <= root_pre) ” 
   &&  “ (root_pre < n_pre) ” 
   &&  “ (0 <= u_pre) ” 
   &&  “ (u_pre < n_pre) ” 
   &&  “ (n_pre <= INT_MAX) ”
-  &&  (SllPtrArray.missing_i fadj_pre n_pre u_pre head fadj_rows_low_level_spec )
-  **  (sllseg head row_ptr processed )
+  &&  (sllseg row_ptr_2 row_ptr processed )
   **  (sll row_ptr rem )
 ).
 
@@ -1142,6 +1187,7 @@ Definition dfs2_entail_wit_2 :=
 (
 forall (sid_pre: Z) (vis2_pre: Z) (fadj_pre: Z) (n_pre: Z) (u_pre: Z) (root_pre: Z) (fadj_rows_low_level_spec: (@list (@list Z))) (X_low_level_spec: (unit -> (KSt -> Prop))) (g_low_level_spec: AdjGraph) (cur: Z) (head: Z) (processed: (@list Z)) (rem: (@list Z)) (vis2_m: (@list Z)) (sid_m: (@list Z)) (PreH1 : (cur <> 0)) (PreH2 : (safeExec (pre_dfs2 (g_low_level_spec) (vis2_m) (sid_m)) (dfs_scc_from (root_pre) (u_pre) ((edges_of (u_pre) (processed)))) X_low_level_spec )) (PreH3 : (0 <= root_pre)) (PreH4 : (root_pre < n_pre)) (PreH5 : (0 <= u_pre)) (PreH6 : (u_pre < n_pre)) (PreH7 : (n_pre <= INT_MAX)) ,
   ((( &( "v" ) )) # Int  |->_)
+  **  (((fadj_pre + (u_pre * sizeof(PTR) ) )) # Ptr  |-> head)
   **  (SllPtrArray.missing_i fadj_pre n_pre u_pre head fadj_rows_low_level_spec )
   **  (sllseg head cur processed )
   **  (sll cur rem )
@@ -1156,6 +1202,7 @@ forall (sid_pre: Z) (vis2_pre: Z) (fadj_pre: Z) (n_pre: Z) (u_pre: Z) (root_pre:
   &&  “ (rem = (cons (vdata) (rest))) ” 
   &&  “ (safeExec (pre_dfs2 (g_low_level_spec) (vis2_m) (sid_m)) (dfs_scc_from (root_pre) (u_pre) ((edges_of (u_pre) (processed)))) X_low_level_spec ) ”
   &&  ((( &( "v" ) )) # Int  |-> vdata)
+  **  (((fadj_pre + (u_pre * sizeof(PTR) ) )) # Ptr  |-> head)
   **  (SllPtrArray.missing_i fadj_pre n_pre u_pre head fadj_rows_low_level_spec )
   **  (sllseg head cur processed )
   **  ((&((cur)  # "list" ->ₛ "data")) # Int  |-> vdata)
@@ -1208,6 +1255,7 @@ forall (sid_pre: Z) (vis2_pre: Z) (fadj_pre: Z) (n_pre: Z) (u_pre: Z) (root_pre:
   **  ((( &( "u" ) )) # Int  |-> u)
   **  ((( &( "root" ) )) # Int  |-> root)
   **  ((( &( "fadj" ) )) # Ptr  |-> fadj)
+  **  (((fadj + (u * sizeof(PTR) ) )) # Ptr  |-> head)
   **  (SllPtrArray.missing_i fadj n u head fadj_rows_low_level_spec )
   **  (sllseg head cur processed )
   **  ((&((cur)  # "list" ->ₛ "data")) # Int  |-> vdata)
@@ -1240,6 +1288,7 @@ forall (sid_pre: Z) (vis2_pre: Z) (fadj_pre: Z) (n_pre: Z) (u_pre: Z) (root_pre:
 (
 forall (sid_pre: Z) (vis2_pre: Z) (fadj_pre: Z) (n_pre: Z) (u_pre: Z) (root_pre: Z) (fadj_rows_low_level_spec: (@list (@list Z))) (X_low_level_spec: (unit -> (KSt -> Prop))) (g_low_level_spec: AdjGraph) (head: Z) (processed: (@list Z)) (rem: (@list Z)) (vis2_m: (@list Z)) (sid_m: (@list Z)) (vdata: Z) (rest: (@list Z)) (next_ptr: Z) (cur: Z) (n: Z) (u: Z) (root: Z) (fadj: Z) (vis2: Z) (sid: Z) (PreH1 : (vdata <= INT_MAX)) (PreH2 : (vdata >= INT_MIN)) (PreH3 : ((Znth vdata vis2_m 0) = 0)) (PreH4 : (cur <> 0)) (PreH5 : (0 <= vdata)) (PreH6 : (vdata < n)) (PreH7 : (n <= INT_MAX)) (PreH8 : (rem = (cons (vdata) (rest)))) (PreH9 : (safeExec (pre_dfs2 (g_low_level_spec) (vis2_m) (sid_m)) (dfs_scc_from (root) (u) ((edges_of (u) (processed)))) X_low_level_spec )) ,
   (IntArray.full vis2 n vis2_m )
+  **  (((fadj + (u * sizeof(PTR) ) )) # Ptr  |-> head)
   **  (SllPtrArray.missing_i fadj n u head fadj_rows_low_level_spec )
   **  (sllseg head cur processed )
   **  ((&((cur)  # "list" ->ₛ "data")) # Int  |-> vdata)
@@ -1269,6 +1318,7 @@ forall (sid_pre: Z) (vis2_pre: Z) (fadj_pre: Z) (n_pre: Z) (u_pre: Z) (root_pre:
 Definition dfs2_entail_wit_3_split_goal_1 := 
 forall (root_pre: Z) (fadj_rows_low_level_spec: (@list (@list Z))) (X_low_level_spec: (unit -> (KSt -> Prop))) (g_low_level_spec: AdjGraph) (head: Z) (processed: (@list Z)) (rem: (@list Z)) (vis2_m: (@list Z)) (sid_m: (@list Z)) (vdata: Z) (rest: (@list Z)) (next_ptr: Z) (cur: Z) (n: Z) (u: Z) (root: Z) (fadj: Z) (vis2: Z) (sid: Z) (PreH1 : (vdata <= INT_MAX)) (PreH2 : (vdata >= INT_MIN)) (PreH3 : ((Znth vdata vis2_m 0) = 0)) (PreH4 : (cur <> 0)) (PreH5 : (0 <= vdata)) (PreH6 : (vdata < n)) (PreH7 : (n <= INT_MAX)) (PreH8 : (rem = (cons (vdata) (rest)))) (PreH9 : (safeExec (pre_dfs2 (g_low_level_spec) (vis2_m) (sid_m)) (dfs_scc_from (root) (u) ((edges_of (u) (processed)))) X_low_level_spec )) ,
   (IntArray.full vis2 n vis2_m )
+  **  (((fadj + (u * sizeof(PTR) ) )) # Ptr  |-> head)
   **  (SllPtrArray.missing_i fadj n u head fadj_rows_low_level_spec )
   **  (sllseg head cur processed )
   **  ((&((cur)  # "list" ->ₛ "data")) # Int  |-> vdata)
@@ -1282,6 +1332,7 @@ forall (root_pre: Z) (fadj_rows_low_level_spec: (@list (@list Z))) (X_low_level_
 Definition dfs2_entail_wit_3_split_goal_2 := 
 forall (fadj_rows_low_level_spec: (@list (@list Z))) (X_low_level_spec: (unit -> (KSt -> Prop))) (g_low_level_spec: AdjGraph) (head: Z) (processed: (@list Z)) (rem: (@list Z)) (vis2_m: (@list Z)) (sid_m: (@list Z)) (vdata: Z) (rest: (@list Z)) (next_ptr: Z) (cur: Z) (n: Z) (u: Z) (root: Z) (fadj: Z) (vis2: Z) (sid: Z) (PreH1 : (vdata <= INT_MAX)) (PreH2 : (vdata >= INT_MIN)) (PreH3 : ((Znth vdata vis2_m 0) = 0)) (PreH4 : (cur <> 0)) (PreH5 : (0 <= vdata)) (PreH6 : (vdata < n)) (PreH7 : (n <= INT_MAX)) (PreH8 : (rem = (cons (vdata) (rest)))) (PreH9 : (safeExec (pre_dfs2 (g_low_level_spec) (vis2_m) (sid_m)) (dfs_scc_from (root) (u) ((edges_of (u) (processed)))) X_low_level_spec )) ,
   (IntArray.full vis2 n vis2_m )
+  **  (((fadj + (u * sizeof(PTR) ) )) # Ptr  |-> head)
   **  (SllPtrArray.missing_i fadj n u head fadj_rows_low_level_spec )
   **  (sllseg head cur processed )
   **  ((&((cur)  # "list" ->ₛ "data")) # Int  |-> vdata)
@@ -1295,6 +1346,7 @@ forall (fadj_rows_low_level_spec: (@list (@list Z))) (X_low_level_spec: (unit ->
 Definition dfs2_entail_wit_3_split_goal_3 := 
 forall (n_pre: Z) (fadj_rows_low_level_spec: (@list (@list Z))) (X_low_level_spec: (unit -> (KSt -> Prop))) (g_low_level_spec: AdjGraph) (head: Z) (processed: (@list Z)) (rem: (@list Z)) (vis2_m: (@list Z)) (sid_m: (@list Z)) (vdata: Z) (rest: (@list Z)) (next_ptr: Z) (cur: Z) (n: Z) (u: Z) (root: Z) (fadj: Z) (vis2: Z) (sid: Z) (PreH1 : (vdata <= INT_MAX)) (PreH2 : (vdata >= INT_MIN)) (PreH3 : ((Znth vdata vis2_m 0) = 0)) (PreH4 : (cur <> 0)) (PreH5 : (0 <= vdata)) (PreH6 : (vdata < n)) (PreH7 : (n <= INT_MAX)) (PreH8 : (rem = (cons (vdata) (rest)))) (PreH9 : (safeExec (pre_dfs2 (g_low_level_spec) (vis2_m) (sid_m)) (dfs_scc_from (root) (u) ((edges_of (u) (processed)))) X_low_level_spec )) ,
   (IntArray.full vis2 n vis2_m )
+  **  (((fadj + (u * sizeof(PTR) ) )) # Ptr  |-> head)
   **  (SllPtrArray.missing_i fadj n u head fadj_rows_low_level_spec )
   **  (sllseg head cur processed )
   **  ((&((cur)  # "list" ->ₛ "data")) # Int  |-> vdata)
@@ -1308,6 +1360,7 @@ forall (n_pre: Z) (fadj_rows_low_level_spec: (@list (@list Z))) (X_low_level_spe
 Definition dfs2_entail_wit_3_split_goal_4 := 
 forall (n_pre: Z) (fadj_rows_low_level_spec: (@list (@list Z))) (X_low_level_spec: (unit -> (KSt -> Prop))) (g_low_level_spec: AdjGraph) (head: Z) (processed: (@list Z)) (rem: (@list Z)) (vis2_m: (@list Z)) (sid_m: (@list Z)) (vdata: Z) (rest: (@list Z)) (next_ptr: Z) (cur: Z) (n: Z) (u: Z) (root: Z) (fadj: Z) (vis2: Z) (sid: Z) (PreH1 : (vdata <= INT_MAX)) (PreH2 : (vdata >= INT_MIN)) (PreH3 : ((Znth vdata vis2_m 0) = 0)) (PreH4 : (cur <> 0)) (PreH5 : (0 <= vdata)) (PreH6 : (vdata < n)) (PreH7 : (n <= INT_MAX)) (PreH8 : (rem = (cons (vdata) (rest)))) (PreH9 : (safeExec (pre_dfs2 (g_low_level_spec) (vis2_m) (sid_m)) (dfs_scc_from (root) (u) ((edges_of (u) (processed)))) X_low_level_spec )) ,
   (IntArray.full vis2 n vis2_m )
+  **  (((fadj + (u * sizeof(PTR) ) )) # Ptr  |-> head)
   **  (SllPtrArray.missing_i fadj n u head fadj_rows_low_level_spec )
   **  (sllseg head cur processed )
   **  ((&((cur)  # "list" ->ₛ "data")) # Int  |-> vdata)
@@ -1321,6 +1374,7 @@ forall (n_pre: Z) (fadj_rows_low_level_spec: (@list (@list Z))) (X_low_level_spe
 Definition dfs2_entail_wit_3_split_goal_5 := 
 forall (n_pre: Z) (u_pre: Z) (fadj_rows_low_level_spec: (@list (@list Z))) (X_low_level_spec: (unit -> (KSt -> Prop))) (g_low_level_spec: AdjGraph) (head: Z) (processed: (@list Z)) (rem: (@list Z)) (vis2_m: (@list Z)) (sid_m: (@list Z)) (vdata: Z) (rest: (@list Z)) (next_ptr: Z) (cur: Z) (n: Z) (u: Z) (root: Z) (fadj: Z) (vis2: Z) (sid: Z) (PreH1 : (vdata <= INT_MAX)) (PreH2 : (vdata >= INT_MIN)) (PreH3 : ((Znth vdata vis2_m 0) = 0)) (PreH4 : (cur <> 0)) (PreH5 : (0 <= vdata)) (PreH6 : (vdata < n)) (PreH7 : (n <= INT_MAX)) (PreH8 : (rem = (cons (vdata) (rest)))) (PreH9 : (safeExec (pre_dfs2 (g_low_level_spec) (vis2_m) (sid_m)) (dfs_scc_from (root) (u) ((edges_of (u) (processed)))) X_low_level_spec )) ,
   (IntArray.full vis2 n vis2_m )
+  **  (((fadj + (u * sizeof(PTR) ) )) # Ptr  |-> head)
   **  (SllPtrArray.missing_i fadj n u head fadj_rows_low_level_spec )
   **  (sllseg head cur processed )
   **  ((&((cur)  # "list" ->ₛ "data")) # Int  |-> vdata)
@@ -1334,6 +1388,7 @@ forall (n_pre: Z) (u_pre: Z) (fadj_rows_low_level_spec: (@list (@list Z))) (X_lo
 Definition dfs2_entail_wit_3_split_goal_6 := 
 forall (u_pre: Z) (fadj_rows_low_level_spec: (@list (@list Z))) (X_low_level_spec: (unit -> (KSt -> Prop))) (g_low_level_spec: AdjGraph) (head: Z) (processed: (@list Z)) (rem: (@list Z)) (vis2_m: (@list Z)) (sid_m: (@list Z)) (vdata: Z) (rest: (@list Z)) (next_ptr: Z) (cur: Z) (n: Z) (u: Z) (root: Z) (fadj: Z) (vis2: Z) (sid: Z) (PreH1 : (vdata <= INT_MAX)) (PreH2 : (vdata >= INT_MIN)) (PreH3 : ((Znth vdata vis2_m 0) = 0)) (PreH4 : (cur <> 0)) (PreH5 : (0 <= vdata)) (PreH6 : (vdata < n)) (PreH7 : (n <= INT_MAX)) (PreH8 : (rem = (cons (vdata) (rest)))) (PreH9 : (safeExec (pre_dfs2 (g_low_level_spec) (vis2_m) (sid_m)) (dfs_scc_from (root) (u) ((edges_of (u) (processed)))) X_low_level_spec )) ,
   (IntArray.full vis2 n vis2_m )
+  **  (((fadj + (u * sizeof(PTR) ) )) # Ptr  |-> head)
   **  (SllPtrArray.missing_i fadj n u head fadj_rows_low_level_spec )
   **  (sllseg head cur processed )
   **  ((&((cur)  # "list" ->ₛ "data")) # Int  |-> vdata)
@@ -1347,6 +1402,7 @@ forall (u_pre: Z) (fadj_rows_low_level_spec: (@list (@list Z))) (X_low_level_spe
 Definition dfs2_entail_wit_3_split_goal_7 := 
 forall (n_pre: Z) (root_pre: Z) (fadj_rows_low_level_spec: (@list (@list Z))) (X_low_level_spec: (unit -> (KSt -> Prop))) (g_low_level_spec: AdjGraph) (head: Z) (processed: (@list Z)) (rem: (@list Z)) (vis2_m: (@list Z)) (sid_m: (@list Z)) (vdata: Z) (rest: (@list Z)) (next_ptr: Z) (cur: Z) (n: Z) (u: Z) (root: Z) (fadj: Z) (vis2: Z) (sid: Z) (PreH1 : (vdata <= INT_MAX)) (PreH2 : (vdata >= INT_MIN)) (PreH3 : ((Znth vdata vis2_m 0) = 0)) (PreH4 : (cur <> 0)) (PreH5 : (0 <= vdata)) (PreH6 : (vdata < n)) (PreH7 : (n <= INT_MAX)) (PreH8 : (rem = (cons (vdata) (rest)))) (PreH9 : (safeExec (pre_dfs2 (g_low_level_spec) (vis2_m) (sid_m)) (dfs_scc_from (root) (u) ((edges_of (u) (processed)))) X_low_level_spec )) ,
   (IntArray.full vis2 n vis2_m )
+  **  (((fadj + (u * sizeof(PTR) ) )) # Ptr  |-> head)
   **  (SllPtrArray.missing_i fadj n u head fadj_rows_low_level_spec )
   **  (sllseg head cur processed )
   **  ((&((cur)  # "list" ->ₛ "data")) # Int  |-> vdata)
@@ -1360,6 +1416,7 @@ forall (n_pre: Z) (root_pre: Z) (fadj_rows_low_level_spec: (@list (@list Z))) (X
 Definition dfs2_entail_wit_3_split_goal_8 := 
 forall (root_pre: Z) (fadj_rows_low_level_spec: (@list (@list Z))) (X_low_level_spec: (unit -> (KSt -> Prop))) (g_low_level_spec: AdjGraph) (head: Z) (processed: (@list Z)) (rem: (@list Z)) (vis2_m: (@list Z)) (sid_m: (@list Z)) (vdata: Z) (rest: (@list Z)) (next_ptr: Z) (cur: Z) (n: Z) (u: Z) (root: Z) (fadj: Z) (vis2: Z) (sid: Z) (PreH1 : (vdata <= INT_MAX)) (PreH2 : (vdata >= INT_MIN)) (PreH3 : ((Znth vdata vis2_m 0) = 0)) (PreH4 : (cur <> 0)) (PreH5 : (0 <= vdata)) (PreH6 : (vdata < n)) (PreH7 : (n <= INT_MAX)) (PreH8 : (rem = (cons (vdata) (rest)))) (PreH9 : (safeExec (pre_dfs2 (g_low_level_spec) (vis2_m) (sid_m)) (dfs_scc_from (root) (u) ((edges_of (u) (processed)))) X_low_level_spec )) ,
   (IntArray.full vis2 n vis2_m )
+  **  (((fadj + (u * sizeof(PTR) ) )) # Ptr  |-> head)
   **  (SllPtrArray.missing_i fadj n u head fadj_rows_low_level_spec )
   **  (sllseg head cur processed )
   **  ((&((cur)  # "list" ->ₛ "data")) # Int  |-> vdata)
@@ -1373,6 +1430,7 @@ forall (root_pre: Z) (fadj_rows_low_level_spec: (@list (@list Z))) (X_low_level_
 Definition dfs2_entail_wit_3_split_goal_9 := 
 forall (n_pre: Z) (fadj_rows_low_level_spec: (@list (@list Z))) (X_low_level_spec: (unit -> (KSt -> Prop))) (g_low_level_spec: AdjGraph) (head: Z) (processed: (@list Z)) (rem: (@list Z)) (vis2_m: (@list Z)) (sid_m: (@list Z)) (vdata: Z) (rest: (@list Z)) (next_ptr: Z) (cur: Z) (n: Z) (u: Z) (root: Z) (fadj: Z) (vis2: Z) (sid: Z) (PreH1 : (vdata <= INT_MAX)) (PreH2 : (vdata >= INT_MIN)) (PreH3 : ((Znth vdata vis2_m 0) = 0)) (PreH4 : (cur <> 0)) (PreH5 : (0 <= vdata)) (PreH6 : (vdata < n)) (PreH7 : (n <= INT_MAX)) (PreH8 : (rem = (cons (vdata) (rest)))) (PreH9 : (safeExec (pre_dfs2 (g_low_level_spec) (vis2_m) (sid_m)) (dfs_scc_from (root) (u) ((edges_of (u) (processed)))) X_low_level_spec )) ,
   (IntArray.full vis2 n vis2_m )
+  **  (((fadj + (u * sizeof(PTR) ) )) # Ptr  |-> head)
   **  (SllPtrArray.missing_i fadj n u head fadj_rows_low_level_spec )
   **  (sllseg head cur processed )
   **  ((&((cur)  # "list" ->ₛ "data")) # Int  |-> vdata)
@@ -1386,6 +1444,7 @@ forall (n_pre: Z) (fadj_rows_low_level_spec: (@list (@list Z))) (X_low_level_spe
 Definition dfs2_entail_wit_3_split_goal_10 := 
 forall (u_pre: Z) (fadj_rows_low_level_spec: (@list (@list Z))) (X_low_level_spec: (unit -> (KSt -> Prop))) (g_low_level_spec: AdjGraph) (head: Z) (processed: (@list Z)) (rem: (@list Z)) (vis2_m: (@list Z)) (sid_m: (@list Z)) (vdata: Z) (rest: (@list Z)) (next_ptr: Z) (cur: Z) (n: Z) (u: Z) (root: Z) (fadj: Z) (vis2: Z) (sid: Z) (PreH1 : (vdata <= INT_MAX)) (PreH2 : (vdata >= INT_MIN)) (PreH3 : ((Znth vdata vis2_m 0) = 0)) (PreH4 : (cur <> 0)) (PreH5 : (0 <= vdata)) (PreH6 : (vdata < n)) (PreH7 : (n <= INT_MAX)) (PreH8 : (rem = (cons (vdata) (rest)))) (PreH9 : (safeExec (pre_dfs2 (g_low_level_spec) (vis2_m) (sid_m)) (dfs_scc_from (root) (u) ((edges_of (u) (processed)))) X_low_level_spec )) ,
   (IntArray.full vis2 n vis2_m )
+  **  (((fadj + (u * sizeof(PTR) ) )) # Ptr  |-> head)
   **  (SllPtrArray.missing_i fadj n u head fadj_rows_low_level_spec )
   **  (sllseg head cur processed )
   **  ((&((cur)  # "list" ->ₛ "data")) # Int  |-> vdata)
@@ -1399,6 +1458,7 @@ forall (u_pre: Z) (fadj_rows_low_level_spec: (@list (@list Z))) (X_low_level_spe
 Definition dfs2_entail_wit_3_split_goal_11 := 
 forall (root_pre: Z) (fadj_rows_low_level_spec: (@list (@list Z))) (X_low_level_spec: (unit -> (KSt -> Prop))) (g_low_level_spec: AdjGraph) (head: Z) (processed: (@list Z)) (rem: (@list Z)) (vis2_m: (@list Z)) (sid_m: (@list Z)) (vdata: Z) (rest: (@list Z)) (next_ptr: Z) (cur: Z) (n: Z) (u: Z) (root: Z) (fadj: Z) (vis2: Z) (sid: Z) (PreH1 : (vdata <= INT_MAX)) (PreH2 : (vdata >= INT_MIN)) (PreH3 : ((Znth vdata vis2_m 0) = 0)) (PreH4 : (cur <> 0)) (PreH5 : (0 <= vdata)) (PreH6 : (vdata < n)) (PreH7 : (n <= INT_MAX)) (PreH8 : (rem = (cons (vdata) (rest)))) (PreH9 : (safeExec (pre_dfs2 (g_low_level_spec) (vis2_m) (sid_m)) (dfs_scc_from (root) (u) ((edges_of (u) (processed)))) X_low_level_spec )) ,
   (IntArray.full vis2 n vis2_m )
+  **  (((fadj + (u * sizeof(PTR) ) )) # Ptr  |-> head)
   **  (SllPtrArray.missing_i fadj n u head fadj_rows_low_level_spec )
   **  (sllseg head cur processed )
   **  ((&((cur)  # "list" ->ₛ "data")) # Int  |-> vdata)
@@ -1412,6 +1472,7 @@ forall (root_pre: Z) (fadj_rows_low_level_spec: (@list (@list Z))) (X_low_level_
 Definition dfs2_entail_wit_3_split_goal_12 := 
 forall (fadj_pre: Z) (fadj_rows_low_level_spec: (@list (@list Z))) (X_low_level_spec: (unit -> (KSt -> Prop))) (g_low_level_spec: AdjGraph) (head: Z) (processed: (@list Z)) (rem: (@list Z)) (vis2_m: (@list Z)) (sid_m: (@list Z)) (vdata: Z) (rest: (@list Z)) (next_ptr: Z) (cur: Z) (n: Z) (u: Z) (root: Z) (fadj: Z) (vis2: Z) (sid: Z) (PreH1 : (vdata <= INT_MAX)) (PreH2 : (vdata >= INT_MIN)) (PreH3 : ((Znth vdata vis2_m 0) = 0)) (PreH4 : (cur <> 0)) (PreH5 : (0 <= vdata)) (PreH6 : (vdata < n)) (PreH7 : (n <= INT_MAX)) (PreH8 : (rem = (cons (vdata) (rest)))) (PreH9 : (safeExec (pre_dfs2 (g_low_level_spec) (vis2_m) (sid_m)) (dfs_scc_from (root) (u) ((edges_of (u) (processed)))) X_low_level_spec )) ,
   (IntArray.full vis2 n vis2_m )
+  **  (((fadj + (u * sizeof(PTR) ) )) # Ptr  |-> head)
   **  (SllPtrArray.missing_i fadj n u head fadj_rows_low_level_spec )
   **  (sllseg head cur processed )
   **  ((&((cur)  # "list" ->ₛ "data")) # Int  |-> vdata)
@@ -1425,6 +1486,7 @@ forall (fadj_pre: Z) (fadj_rows_low_level_spec: (@list (@list Z))) (X_low_level_
 Definition dfs2_entail_wit_3_split_goal_13 := 
 forall (vis2_pre: Z) (fadj_rows_low_level_spec: (@list (@list Z))) (X_low_level_spec: (unit -> (KSt -> Prop))) (g_low_level_spec: AdjGraph) (head: Z) (processed: (@list Z)) (rem: (@list Z)) (vis2_m: (@list Z)) (sid_m: (@list Z)) (vdata: Z) (rest: (@list Z)) (next_ptr: Z) (cur: Z) (n: Z) (u: Z) (root: Z) (fadj: Z) (vis2: Z) (sid: Z) (PreH1 : (vdata <= INT_MAX)) (PreH2 : (vdata >= INT_MIN)) (PreH3 : ((Znth vdata vis2_m 0) = 0)) (PreH4 : (cur <> 0)) (PreH5 : (0 <= vdata)) (PreH6 : (vdata < n)) (PreH7 : (n <= INT_MAX)) (PreH8 : (rem = (cons (vdata) (rest)))) (PreH9 : (safeExec (pre_dfs2 (g_low_level_spec) (vis2_m) (sid_m)) (dfs_scc_from (root) (u) ((edges_of (u) (processed)))) X_low_level_spec )) ,
   (IntArray.full vis2 n vis2_m )
+  **  (((fadj + (u * sizeof(PTR) ) )) # Ptr  |-> head)
   **  (SllPtrArray.missing_i fadj n u head fadj_rows_low_level_spec )
   **  (sllseg head cur processed )
   **  ((&((cur)  # "list" ->ₛ "data")) # Int  |-> vdata)
@@ -1438,6 +1500,7 @@ forall (vis2_pre: Z) (fadj_rows_low_level_spec: (@list (@list Z))) (X_low_level_
 Definition dfs2_entail_wit_3_split_goal_14 := 
 forall (sid_pre: Z) (fadj_rows_low_level_spec: (@list (@list Z))) (X_low_level_spec: (unit -> (KSt -> Prop))) (g_low_level_spec: AdjGraph) (head: Z) (processed: (@list Z)) (rem: (@list Z)) (vis2_m: (@list Z)) (sid_m: (@list Z)) (vdata: Z) (rest: (@list Z)) (next_ptr: Z) (cur: Z) (n: Z) (u: Z) (root: Z) (fadj: Z) (vis2: Z) (sid: Z) (PreH1 : (vdata <= INT_MAX)) (PreH2 : (vdata >= INT_MIN)) (PreH3 : ((Znth vdata vis2_m 0) = 0)) (PreH4 : (cur <> 0)) (PreH5 : (0 <= vdata)) (PreH6 : (vdata < n)) (PreH7 : (n <= INT_MAX)) (PreH8 : (rem = (cons (vdata) (rest)))) (PreH9 : (safeExec (pre_dfs2 (g_low_level_spec) (vis2_m) (sid_m)) (dfs_scc_from (root) (u) ((edges_of (u) (processed)))) X_low_level_spec )) ,
   (IntArray.full vis2 n vis2_m )
+  **  (((fadj + (u * sizeof(PTR) ) )) # Ptr  |-> head)
   **  (SllPtrArray.missing_i fadj n u head fadj_rows_low_level_spec )
   **  (sllseg head cur processed )
   **  ((&((cur)  # "list" ->ₛ "data")) # Int  |-> vdata)
@@ -1451,6 +1514,7 @@ forall (sid_pre: Z) (fadj_rows_low_level_spec: (@list (@list Z))) (X_low_level_s
 Definition dfs2_entail_wit_3_split_goal_spatial := 
 forall (sid_pre: Z) (vis2_pre: Z) (fadj_pre: Z) (n_pre: Z) (fadj_rows_low_level_spec: (@list (@list Z))) (X_low_level_spec: (unit -> (KSt -> Prop))) (g_low_level_spec: AdjGraph) (head: Z) (processed: (@list Z)) (rem: (@list Z)) (vis2_m: (@list Z)) (sid_m: (@list Z)) (vdata: Z) (rest: (@list Z)) (next_ptr: Z) (cur: Z) (n: Z) (u: Z) (root: Z) (fadj: Z) (vis2: Z) (sid: Z) (PreH1 : (vdata <= INT_MAX)) (PreH2 : (vdata >= INT_MIN)) (PreH3 : ((Znth vdata vis2_m 0) = 0)) (PreH4 : (cur <> 0)) (PreH5 : (0 <= vdata)) (PreH6 : (vdata < n)) (PreH7 : (n <= INT_MAX)) (PreH8 : (rem = (cons (vdata) (rest)))) (PreH9 : (safeExec (pre_dfs2 (g_low_level_spec) (vis2_m) (sid_m)) (dfs_scc_from (root) (u) ((edges_of (u) (processed)))) X_low_level_spec )) ,
   (IntArray.full vis2 n vis2_m )
+  **  (((fadj + (u * sizeof(PTR) ) )) # Ptr  |-> head)
   **  (SllPtrArray.missing_i fadj n u head fadj_rows_low_level_spec )
   **  (sllseg head cur processed )
   **  ((&((cur)  # "list" ->ₛ "data")) # Int  |-> vdata)
@@ -1471,6 +1535,7 @@ forall (sid_pre: Z) (vis2_pre: Z) (fadj_pre: Z) (n_pre: Z) (u_pre: Z) (root_pre:
   **  ((( &( "u" ) )) # Int  |-> u)
   **  ((( &( "root" ) )) # Int  |-> root)
   **  ((( &( "fadj" ) )) # Ptr  |-> fadj)
+  **  (((fadj + (u * sizeof(PTR) ) )) # Ptr  |-> head)
   **  (SllPtrArray.missing_i fadj n u head fadj_rows_low_level_spec )
   **  (sllseg head cur processed )
   **  ((&((cur)  # "list" ->ₛ "data")) # Int  |-> vdata)
@@ -1495,6 +1560,7 @@ forall (sid_pre: Z) (vis2_pre: Z) (fadj_pre: Z) (n_pre: Z) (u_pre: Z) (root_pre:
   **  ((( &( "fadj" ) )) # Ptr  |-> fadj_pre)
   **  ((( &( "vis2" ) )) # Ptr  |-> vis2_pre)
   **  ((( &( "sid" ) )) # Ptr  |-> sid_pre)
+  **  (((fadj_pre + (u_pre * sizeof(PTR) ) )) # Ptr  |-> head)
   **  (SllPtrArray.missing_i fadj_pre n_pre u_pre head fadj_rows_low_level_spec )
   **  (sllseg head cur processed )
   **  ((&((cur)  # "list" ->ₛ "data")) # Int  |-> vdata)
@@ -1506,6 +1572,7 @@ forall (sid_pre: Z) (vis2_pre: Z) (fadj_pre: Z) (n_pre: Z) (u_pre: Z) (root_pre:
 (
 forall (sid_pre: Z) (vis2_pre: Z) (fadj_pre: Z) (n_pre: Z) (u_pre: Z) (root_pre: Z) (fadj_rows_low_level_spec: (@list (@list Z))) (X_low_level_spec: (unit -> (KSt -> Prop))) (g_low_level_spec: AdjGraph) (head: Z) (processed: (@list Z)) (rem: (@list Z)) (vis2_m: (@list Z)) (sid_m: (@list Z)) (vdata: Z) (rest: (@list Z)) (cur: Z) (n: Z) (u: Z) (root: Z) (fadj: Z) (vis2: Z) (sid: Z) (PreH1 : ((Znth vdata vis2_m 0) <> 0)) (PreH2 : (cur <> 0)) (PreH3 : (0 <= vdata)) (PreH4 : (vdata < n)) (PreH5 : (n <= INT_MAX)) (PreH6 : (rem = (cons (vdata) (rest)))) (PreH7 : (safeExec (pre_dfs2 (g_low_level_spec) (vis2_m) (sid_m)) (dfs_scc_from (root) (u) ((edges_of (u) (processed)))) X_low_level_spec )) ,
   (IntArray.full vis2 n vis2_m )
+  **  (((fadj + (u * sizeof(PTR) ) )) # Ptr  |-> head)
   **  (SllPtrArray.missing_i fadj n u head fadj_rows_low_level_spec )
   **  (sllseg head cur processed )
   **  (IntArray.full sid n sid_m )
@@ -1525,7 +1592,8 @@ forall (sid_pre: Z) (vis2_pre: Z) (fadj_pre: Z) (n_pre: Z) (u_pre: Z) (root_pre:
   &&  “ (n_pre <= INT_MAX) ” 
   &&  “ (rem = (cons (vdata) (rest))) ” 
   &&  “ (safeExec (pre_dfs2 (g_low_level_spec) (vis2_m_) (sid_m_)) (dfs_scc_from (root_pre) (u_pre) ((edges_of (u_pre) (processed)))) X_low_level_spec ) ”
-  &&  (SllPtrArray.missing_i fadj_pre n_pre u_pre head fadj_rows_low_level_spec )
+  &&  (((fadj_pre + (u_pre * sizeof(PTR) ) )) # Ptr  |-> head)
+  **  (SllPtrArray.missing_i fadj_pre n_pre u_pre head fadj_rows_low_level_spec )
   **  (sllseg head cur processed )
   **  (IntArray.full vis2_pre n_pre vis2_m_ )
   **  (IntArray.full sid_pre n_pre sid_m_ )
@@ -1547,7 +1615,8 @@ forall (sid_pre: Z) (vis2_pre: Z) (fadj_pre: Z) (n_pre: Z) (u_pre: Z) (root_pre:
   &&  “ (n_pre <= INT_MAX) ” 
   &&  “ (rem = (cons (v) (rest_))) ” 
   &&  “ (safeExec (pre_dfs2 (g_low_level_spec) (vis2_m_) (sid_m_)) (dfs_scc_from (root_pre) (u_pre) ((edges_of (u_pre) (processed)))) X_low_level_spec ) ”
-  &&  (SllPtrArray.missing_i fadj_pre n_pre u_pre head fadj_rows_low_level_spec )
+  &&  (((fadj_pre + (u_pre * sizeof(PTR) ) )) # Ptr  |-> head)
+  **  (SllPtrArray.missing_i fadj_pre n_pre u_pre head fadj_rows_low_level_spec )
   **  (sllseg head cur processed )
   **  ((&((cur)  # "list" ->ₛ "data")) # Int  |-> v)
   **  ((&((cur)  # "list" ->ₛ "next")) # Ptr  |-> next_ptr_)
@@ -1556,11 +1625,13 @@ forall (sid_pre: Z) (vis2_pre: Z) (fadj_pre: Z) (n_pre: Z) (u_pre: Z) (root_pre:
   **  (IntArray.full sid_pre n_pre sid_m_ )
 ) \/
 (
-forall (fadj_pre: Z) (n_pre: Z) (u_pre: Z) (root_pre: Z) (fadj_rows_low_level_spec: (@list (@list Z))) (X_low_level_spec: (unit -> (KSt -> Prop))) (g_low_level_spec: AdjGraph) (head: Z) (processed: (@list Z)) (rem: (@list Z)) (vis2_m: (@list Z)) (cur: Z) (v: Z) (vis2_l_: (@list Z)) (sid_l_: (@list Z)) (PreH1 : (safeExec (pre_dfs2 (g_low_level_spec) (vis2_l_) (sid_l_)) (return (tt)) X_low_level_spec )) (PreH2 : (cur <> 0)) (PreH3 : (0 <= root_pre)) (PreH4 : (root_pre < n_pre)) (PreH5 : (0 <= u_pre)) (PreH6 : (u_pre < n_pre)) (PreH7 : (0 <= v)) (PreH8 : (v < n_pre)) (PreH9 : (n_pre <= INT_MAX)) (PreH10 : ((Znth (v) (vis2_m) (0)) = 0)) ,
-  (SllPtrArray.full fadj_pre n_pre fadj_rows_low_level_spec )
+forall (fadj_pre: Z) (n_pre: Z) (u_pre: Z) (root_pre: Z) (fadj_rows_low_level_spec: (@list (@list Z))) (X_low_level_spec: (unit -> (KSt -> Prop))) (g_low_level_spec: AdjGraph) (head: Z) (processed: (@list Z)) (rem: (@list Z)) (vis2_m: (@list Z)) (cur: Z) (v: Z) (vis2_l_: (@list Z)) (sid_l_: (@list Z)) (row_ptr: Z)  __default__List_Z (PreH1 : (safeExec (pre_dfs2 (g_low_level_spec) (vis2_l_) (sid_l_)) (return (tt)) X_low_level_spec )) (PreH2 : (cur <> 0)) (PreH3 : (0 <= root_pre)) (PreH4 : (root_pre < n_pre)) (PreH5 : (0 <= u_pre)) (PreH6 : (u_pre < n_pre)) (PreH7 : (0 <= v)) (PreH8 : (v < n_pre)) (PreH9 : (n_pre <= INT_MAX)) (PreH10 : ((Znth (v) (vis2_m) (0)) = 0)) ,
+  (sll row_ptr (Znth u_pre fadj_rows_low_level_spec __default__List_Z) )
+  **  (SllPtrArray.missing_i fadj_pre n_pre u_pre row_ptr fadj_rows_low_level_spec )
 |--
   EX (next_ptr_: Z)  (rest_: (@list Z)) ,
-  “ (cur <> 0) ” 
+  “ (head = row_ptr) ” 
+  &&  “ (cur <> 0) ” 
   &&  “ (0 <= root_pre) ” 
   &&  “ (root_pre < n_pre) ” 
   &&  “ (0 <= u_pre) ” 
@@ -1578,7 +1649,8 @@ forall (fadj_pre: Z) (n_pre: Z) (u_pre: Z) (root_pre: Z) (fadj_rows_low_level_sp
 Definition dfs2_entail_wit_5 := 
 (
 forall (sid_pre: Z) (vis2_pre: Z) (fadj_pre: Z) (n_pre: Z) (u_pre: Z) (root_pre: Z) (fadj_rows_low_level_spec: (@list (@list Z))) (X_low_level_spec: (unit -> (KSt -> Prop))) (g_low_level_spec: AdjGraph) (head_2: Z) (processed_2: (@list Z)) (rem_2: (@list Z)) (vdata_: Z) (rest_: (@list Z)) (next_ptr_: Z) (vis2_m_: (@list Z)) (sid_m_: (@list Z)) (cur: Z) (PreH1 : (cur <> 0)) (PreH2 : (0 <= root_pre)) (PreH3 : (root_pre < n_pre)) (PreH4 : (0 <= u_pre)) (PreH5 : (u_pre < n_pre)) (PreH6 : (n_pre <= INT_MAX)) (PreH7 : (rem_2 = (cons (vdata_) (rest_)))) (PreH8 : (safeExec (pre_dfs2 (g_low_level_spec) (vis2_m_) (sid_m_)) (dfs_scc_from (root_pre) (u_pre) ((edges_of (u_pre) (processed_2)))) X_low_level_spec )) ,
-  (SllPtrArray.missing_i fadj_pre n_pre u_pre head_2 fadj_rows_low_level_spec )
+  (((fadj_pre + (u_pre * sizeof(PTR) ) )) # Ptr  |-> head_2)
+  **  (SllPtrArray.missing_i fadj_pre n_pre u_pre head_2 fadj_rows_low_level_spec )
   **  (sllseg head_2 cur processed_2 )
   **  ((&((cur)  # "list" ->ₛ "data")) # Int  |-> vdata_)
   **  ((&((cur)  # "list" ->ₛ "next")) # Ptr  |-> next_ptr_)
@@ -1593,34 +1665,34 @@ forall (sid_pre: Z) (vis2_pre: Z) (fadj_pre: Z) (n_pre: Z) (u_pre: Z) (root_pre:
   &&  “ (0 <= u_pre) ” 
   &&  “ (u_pre < n_pre) ” 
   &&  “ (n_pre <= INT_MAX) ”
-  &&  (SllPtrArray.missing_i fadj_pre n_pre u_pre head fadj_rows_low_level_spec )
+  &&  (((fadj_pre + (u_pre * sizeof(PTR) ) )) # Ptr  |-> head)
+  **  (SllPtrArray.missing_i fadj_pre n_pre u_pre head fadj_rows_low_level_spec )
   **  (sllseg head next_ptr_ processed )
   **  (sll next_ptr_ rem )
   **  (IntArray.full vis2_pre n_pre vis2_m )
   **  (IntArray.full sid_pre n_pre sid_m )
 ) \/
 (
-forall (fadj_pre: Z) (n_pre: Z) (u_pre: Z) (root_pre: Z) (fadj_rows_low_level_spec: (@list (@list Z))) (X_low_level_spec: (unit -> (KSt -> Prop))) (g_low_level_spec: AdjGraph) (head_2: Z) (processed_2: (@list Z)) (rem_2: (@list Z)) (vdata_: Z) (rest_: (@list Z)) (next_ptr_: Z) (vis2_m_: (@list Z)) (sid_m_: (@list Z)) (cur: Z) (PreH1 : (vdata_ <= INT_MAX)) (PreH2 : (vdata_ >= INT_MIN)) (PreH3 : (cur <> 0)) (PreH4 : (0 <= root_pre)) (PreH5 : (root_pre < n_pre)) (PreH6 : (0 <= u_pre)) (PreH7 : (u_pre < n_pre)) (PreH8 : (n_pre <= INT_MAX)) (PreH9 : (rem_2 = (cons (vdata_) (rest_)))) (PreH10 : (safeExec (pre_dfs2 (g_low_level_spec) (vis2_m_) (sid_m_)) (dfs_scc_from (root_pre) (u_pre) ((edges_of (u_pre) (processed_2)))) X_low_level_spec )) ,
-  (SllPtrArray.missing_i fadj_pre n_pre u_pre head_2 fadj_rows_low_level_spec )
-  **  (sllseg head_2 cur processed_2 )
+forall (n_pre: Z) (u_pre: Z) (root_pre: Z) (X_low_level_spec: (unit -> (KSt -> Prop))) (g_low_level_spec: AdjGraph) (head_2: Z) (processed_2: (@list Z)) (rem_2: (@list Z)) (vdata_: Z) (rest_: (@list Z)) (next_ptr_: Z) (vis2_m_: (@list Z)) (sid_m_: (@list Z)) (cur: Z) (PreH1 : (vdata_ <= INT_MAX)) (PreH2 : (vdata_ >= INT_MIN)) (PreH3 : (cur <> 0)) (PreH4 : (0 <= root_pre)) (PreH5 : (root_pre < n_pre)) (PreH6 : (0 <= u_pre)) (PreH7 : (u_pre < n_pre)) (PreH8 : (n_pre <= INT_MAX)) (PreH9 : (rem_2 = (cons (vdata_) (rest_)))) (PreH10 : (safeExec (pre_dfs2 (g_low_level_spec) (vis2_m_) (sid_m_)) (dfs_scc_from (root_pre) (u_pre) ((edges_of (u_pre) (processed_2)))) X_low_level_spec )) ,
+  (sllseg head_2 cur processed_2 )
   **  ((&((cur)  # "list" ->ₛ "data")) # Int  |-> vdata_)
   **  ((&((cur)  # "list" ->ₛ "next")) # Ptr  |-> next_ptr_)
 |--
-  EX (head: Z)  (processed: (@list Z)) ,
+  EX (processed: (@list Z)) ,
   “ (safeExec (pre_dfs2 (g_low_level_spec) (vis2_m_) (sid_m_)) (dfs_scc_from (root_pre) (u_pre) ((edges_of (u_pre) (processed)))) X_low_level_spec ) ” 
   &&  “ (0 <= root_pre) ” 
   &&  “ (root_pre < n_pre) ” 
   &&  “ (0 <= u_pre) ” 
   &&  “ (u_pre < n_pre) ” 
   &&  “ (n_pre <= INT_MAX) ”
-  &&  (SllPtrArray.missing_i fadj_pre n_pre u_pre head fadj_rows_low_level_spec )
-  **  (sllseg head next_ptr_ processed )
+  &&  (sllseg head_2 next_ptr_ processed )
 ).
 
 Definition dfs2_entail_wit_6 := 
 (
 forall (sid_pre: Z) (vis2_pre: Z) (fadj_pre: Z) (n_pre: Z) (u_pre: Z) (root_pre: Z) (fadj_rows_low_level_spec: (@list (@list Z))) (X_low_level_spec: (unit -> (KSt -> Prop))) (g_low_level_spec: AdjGraph) (rem: (@list Z)) (cur: Z) (head_2: Z) (vis2_m_2: (@list Z)) (sid_m_2: (@list Z)) (processed: (@list Z)) (PreH1 : (cur = 0)) (PreH2 : (safeExec (pre_dfs2 (g_low_level_spec) (vis2_m_2) (sid_m_2)) (dfs_scc_from (root_pre) (u_pre) ((edges_of (u_pre) (processed)))) X_low_level_spec )) (PreH3 : (0 <= root_pre)) (PreH4 : (root_pre < n_pre)) (PreH5 : (0 <= u_pre)) (PreH6 : (u_pre < n_pre)) (PreH7 : (n_pre <= INT_MAX)) ,
-  (SllPtrArray.missing_i fadj_pre n_pre u_pre head_2 fadj_rows_low_level_spec )
+  (((fadj_pre + (u_pre * sizeof(PTR) ) )) # Ptr  |-> head_2)
+  **  (SllPtrArray.missing_i fadj_pre n_pre u_pre head_2 fadj_rows_low_level_spec )
   **  ((( &( "cur" ) )) # Ptr  |-> cur)
   **  (sllseg head_2 cur processed )
   **  (sll cur rem )
@@ -1634,34 +1706,43 @@ forall (sid_pre: Z) (vis2_pre: Z) (fadj_pre: Z) (n_pre: Z) (u_pre: Z) (root_pre:
   &&  “ (u_pre < n_pre) ” 
   &&  “ (n_pre <= INT_MAX) ” 
   &&  “ (safeExec (pre_dfs2 (g_low_level_spec) (vis2_m) (sid_m)) (return (tt)) X_low_level_spec ) ”
-  &&  (SllPtrArray.missing_i fadj_pre n_pre u_pre head fadj_rows_low_level_spec )
+  &&  (((fadj_pre + (u_pre * sizeof(PTR) ) )) # Ptr  |-> head)
+  **  (SllPtrArray.missing_i fadj_pre n_pre u_pre head fadj_rows_low_level_spec )
   **  (sll head (Znth (u_pre) (fadj_rows_low_level_spec) ((@nil Z))) )
   **  ((( &( "cur" ) )) # Ptr  |-> 0)
   **  (IntArray.full vis2_pre n_pre vis2_m )
   **  (IntArray.full sid_pre n_pre sid_m )
 ) \/
 (
-forall (fadj_pre: Z) (n_pre: Z) (u_pre: Z) (root_pre: Z) (fadj_rows_low_level_spec: (@list (@list Z))) (X_low_level_spec: (unit -> (KSt -> Prop))) (g_low_level_spec: AdjGraph) (rem: (@list Z)) (cur: Z) (head_2: Z) (vis2_m_2: (@list Z)) (sid_m_2: (@list Z)) (processed: (@list Z)) (PreH1 : (cur = 0)) (PreH2 : (safeExec (pre_dfs2 (g_low_level_spec) (vis2_m_2) (sid_m_2)) (dfs_scc_from (root_pre) (u_pre) ((edges_of (u_pre) (processed)))) X_low_level_spec )) (PreH3 : (0 <= root_pre)) (PreH4 : (root_pre < n_pre)) (PreH5 : (0 <= u_pre)) (PreH6 : (u_pre < n_pre)) (PreH7 : (n_pre <= INT_MAX)) ,
-  (SllPtrArray.missing_i fadj_pre n_pre u_pre head_2 fadj_rows_low_level_spec )
-  **  (sllseg head_2 cur processed )
+forall (n_pre: Z) (u_pre: Z) (root_pre: Z) (fadj_rows_low_level_spec: (@list (@list Z))) (X_low_level_spec: (unit -> (KSt -> Prop))) (g_low_level_spec: AdjGraph) (rem: (@list Z)) (cur: Z) (head_2: Z) (vis2_m_2: (@list Z)) (sid_m_2: (@list Z)) (processed: (@list Z)) (PreH1 : (cur = 0)) (PreH2 : (safeExec (pre_dfs2 (g_low_level_spec) (vis2_m_2) (sid_m_2)) (dfs_scc_from (root_pre) (u_pre) ((edges_of (u_pre) (processed)))) X_low_level_spec )) (PreH3 : (0 <= root_pre)) (PreH4 : (root_pre < n_pre)) (PreH5 : (0 <= u_pre)) (PreH6 : (u_pre < n_pre)) (PreH7 : (n_pre <= INT_MAX)) ,
+  (sllseg head_2 cur processed )
   **  (sll cur rem )
 |--
-  EX (head: Z) ,
-  “ (cur = 0) ” 
-  &&  “ (0 <= root_pre) ” 
-  &&  “ (root_pre < n_pre) ” 
-  &&  “ (0 <= u_pre) ” 
-  &&  “ (u_pre < n_pre) ” 
-  &&  “ (n_pre <= INT_MAX) ” 
-  &&  “ (safeExec (pre_dfs2 (g_low_level_spec) (vis2_m_2) (sid_m_2)) (return (tt)) X_low_level_spec ) ”
-  &&  (SllPtrArray.missing_i fadj_pre n_pre u_pre head fadj_rows_low_level_spec )
-  **  (sll head (Znth (u_pre) (fadj_rows_low_level_spec) ((@nil Z))) )
+  “ (safeExec (pre_dfs2 (g_low_level_spec) (vis2_m_2) (sid_m_2)) (return (tt)) X_low_level_spec ) ”
+  &&  (sll head_2 (Znth (u_pre) (fadj_rows_low_level_spec) ((@nil Z))) )
 ).
+
+Definition dfs2_entail_wit_6_split_goal_1 := 
+forall (n_pre: Z) (u_pre: Z) (root_pre: Z) (X_low_level_spec: (unit -> (KSt -> Prop))) (g_low_level_spec: AdjGraph) (rem: (@list Z)) (cur: Z) (head_2: Z) (vis2_m_2: (@list Z)) (sid_m_2: (@list Z)) (processed: (@list Z)) (PreH1 : (cur = 0)) (PreH2 : (safeExec (pre_dfs2 (g_low_level_spec) (vis2_m_2) (sid_m_2)) (dfs_scc_from (root_pre) (u_pre) ((edges_of (u_pre) (processed)))) X_low_level_spec )) (PreH3 : (0 <= root_pre)) (PreH4 : (root_pre < n_pre)) (PreH5 : (0 <= u_pre)) (PreH6 : (u_pre < n_pre)) (PreH7 : (n_pre <= INT_MAX)) ,
+  (sllseg head_2 cur processed )
+  **  (sll cur rem )
+|--
+  “ (safeExec (pre_dfs2 (g_low_level_spec) (vis2_m_2) (sid_m_2)) (return (tt)) X_low_level_spec ) ”
+.
+
+Definition dfs2_entail_wit_6_split_goal_spatial := 
+forall (n_pre: Z) (u_pre: Z) (root_pre: Z) (fadj_rows_low_level_spec: (@list (@list Z))) (X_low_level_spec: (unit -> (KSt -> Prop))) (g_low_level_spec: AdjGraph) (rem: (@list Z)) (cur: Z) (head_2: Z) (vis2_m_2: (@list Z)) (sid_m_2: (@list Z)) (processed: (@list Z)) (PreH1 : (cur = 0)) (PreH2 : (safeExec (pre_dfs2 (g_low_level_spec) (vis2_m_2) (sid_m_2)) (dfs_scc_from (root_pre) (u_pre) ((edges_of (u_pre) (processed)))) X_low_level_spec )) (PreH3 : (0 <= root_pre)) (PreH4 : (root_pre < n_pre)) (PreH5 : (0 <= u_pre)) (PreH6 : (u_pre < n_pre)) (PreH7 : (n_pre <= INT_MAX)) ,
+  (sllseg head_2 cur processed )
+  **  (sll cur rem )
+|--
+  (sll head_2 (Znth (u_pre) (fadj_rows_low_level_spec) ((@nil Z))) )
+.
 
 Definition dfs2_return_wit_1 := 
 (
 forall (sid_pre: Z) (vis2_pre: Z) (fadj_pre: Z) (n_pre: Z) (u_pre: Z) (root_pre: Z) (fadj_rows_low_level_spec: (@list (@list Z))) (X_low_level_spec: (unit -> (KSt -> Prop))) (g_low_level_spec: AdjGraph) (head: Z) (vis2_m: (@list Z)) (sid_m: (@list Z)) (PreH1 : (0 <= root_pre)) (PreH2 : (root_pre < n_pre)) (PreH3 : (0 <= u_pre)) (PreH4 : (u_pre < n_pre)) (PreH5 : (n_pre <= INT_MAX)) (PreH6 : (safeExec (pre_dfs2 (g_low_level_spec) (vis2_m) (sid_m)) (return (tt)) X_low_level_spec )) ,
-  (SllPtrArray.missing_i fadj_pre n_pre u_pre head fadj_rows_low_level_spec )
+  (((fadj_pre + (u_pre * sizeof(PTR) ) )) # Ptr  |-> head)
+  **  (SllPtrArray.missing_i fadj_pre n_pre u_pre head fadj_rows_low_level_spec )
   **  (sll head (Znth (u_pre) (fadj_rows_low_level_spec) ((@nil Z))) )
   **  (IntArray.full vis2_pre n_pre vis2_m )
   **  (IntArray.full sid_pre n_pre sid_m )
@@ -1674,7 +1755,8 @@ forall (sid_pre: Z) (vis2_pre: Z) (fadj_pre: Z) (n_pre: Z) (u_pre: Z) (root_pre:
 ) \/
 (
 forall (fadj_pre: Z) (n_pre: Z) (u_pre: Z) (root_pre: Z) (fadj_rows_low_level_spec: (@list (@list Z))) (X_low_level_spec: (unit -> (KSt -> Prop))) (g_low_level_spec: AdjGraph) (head: Z) (vis2_m: (@list Z)) (sid_m: (@list Z)) (PreH1 : (0 <= root_pre)) (PreH2 : (root_pre < n_pre)) (PreH3 : (0 <= u_pre)) (PreH4 : (u_pre < n_pre)) (PreH5 : (n_pre <= INT_MAX)) (PreH6 : (safeExec (pre_dfs2 (g_low_level_spec) (vis2_m) (sid_m)) (return (tt)) X_low_level_spec )) ,
-  (SllPtrArray.missing_i fadj_pre n_pre u_pre head fadj_rows_low_level_spec )
+  (((fadj_pre + (u_pre * sizeof(PTR) ) )) # Ptr  |-> head)
+  **  (SllPtrArray.missing_i fadj_pre n_pre u_pre head fadj_rows_low_level_spec )
   **  (sll head (Znth (u_pre) (fadj_rows_low_level_spec) ((@nil Z))) )
 |--
   (SllPtrArray.full fadj_pre n_pre fadj_rows_low_level_spec )
@@ -1682,7 +1764,8 @@ forall (fadj_pre: Z) (n_pre: Z) (u_pre: Z) (root_pre: Z) (fadj_rows_low_level_sp
 
 Definition dfs2_return_wit_1_split_goal_spatial := 
 forall (fadj_pre: Z) (n_pre: Z) (u_pre: Z) (root_pre: Z) (fadj_rows_low_level_spec: (@list (@list Z))) (X_low_level_spec: (unit -> (KSt -> Prop))) (g_low_level_spec: AdjGraph) (head: Z) (vis2_m: (@list Z)) (sid_m: (@list Z)) (PreH1 : (0 <= root_pre)) (PreH2 : (root_pre < n_pre)) (PreH3 : (0 <= u_pre)) (PreH4 : (u_pre < n_pre)) (PreH5 : (n_pre <= INT_MAX)) (PreH6 : (safeExec (pre_dfs2 (g_low_level_spec) (vis2_m) (sid_m)) (return (tt)) X_low_level_spec )) ,
-  (SllPtrArray.missing_i fadj_pre n_pre u_pre head fadj_rows_low_level_spec )
+  (((fadj_pre + (u_pre * sizeof(PTR) ) )) # Ptr  |-> head)
+  **  (SllPtrArray.missing_i fadj_pre n_pre u_pre head fadj_rows_low_level_spec )
   **  (sll head (Znth (u_pre) (fadj_rows_low_level_spec) ((@nil Z))) )
 |--
   (SllPtrArray.full fadj_pre n_pre fadj_rows_low_level_spec )
@@ -1764,7 +1847,8 @@ forall (sid_pre: Z) (vis2_pre: Z) (fadj_pre: Z) (n_pre: Z) (u_pre: Z) (root_pre:
 
 Definition dfs2_partial_solve_wit_5 := 
 forall (fadj_rows_low_level_spec: (@list (@list Z))) (X_low_level_spec: (unit -> (KSt -> Prop))) (g_low_level_spec: AdjGraph) (head: Z) (processed: (@list Z)) (rem: (@list Z)) (vis2_m: (@list Z)) (sid_m: (@list Z)) (vdata: Z) (rest: (@list Z)) (next_ptr: Z) (cur: Z) (n: Z) (u: Z) (root: Z) (fadj: Z) (vis2: Z) (sid: Z) (PreH1 : (cur <> 0)) (PreH2 : (0 <= vdata)) (PreH3 : (vdata < n)) (PreH4 : (n <= INT_MAX)) (PreH5 : (rem = (cons (vdata) (rest)))) (PreH6 : (safeExec (pre_dfs2 (g_low_level_spec) (vis2_m) (sid_m)) (dfs_scc_from (root) (u) ((edges_of (u) (processed)))) X_low_level_spec )) ,
-  (SllPtrArray.missing_i fadj n u head fadj_rows_low_level_spec )
+  (((fadj + (u * sizeof(PTR) ) )) # Ptr  |-> head)
+  **  (SllPtrArray.missing_i fadj n u head fadj_rows_low_level_spec )
   **  (sllseg head cur processed )
   **  ((&((cur)  # "list" ->ₛ "data")) # Int  |-> vdata)
   **  ((&((cur)  # "list" ->ₛ "next")) # Ptr  |-> next_ptr)
@@ -1780,6 +1864,7 @@ forall (fadj_rows_low_level_spec: (@list (@list Z))) (X_low_level_spec: (unit ->
   &&  “ (safeExec (pre_dfs2 (g_low_level_spec) (vis2_m) (sid_m)) (dfs_scc_from (root) (u) ((edges_of (u) (processed)))) X_low_level_spec ) ”
   &&  (((vis2 + (vdata * sizeof(INT) ) )) # Int  |-> (Znth vdata vis2_m 0))
   **  (IntArray.missing_i vis2 vdata 0 n vis2_m )
+  **  (((fadj + (u * sizeof(PTR) ) )) # Ptr  |-> head)
   **  (SllPtrArray.missing_i fadj n u head fadj_rows_low_level_spec )
   **  (sllseg head cur processed )
   **  ((&((cur)  # "list" ->ₛ "data")) # Int  |-> vdata)
